WIP

src/example/TicketLockW.v
@@ -86,7 +86,2290 @@ From Fairness Require Import IProp IPM Weakest.
 From Fairness Require Import ModSim PCM MonotonePCM StateRA FairRA.
 From Fairness Require Import FairLock.
 
+Section AUX.
+
+  Variant prod_le
+          {A B: Type} {RA: A -> A -> Prop} {RB: B -> B -> Prop}
+          (PRA: PartialOrder RA) (PRB: PreOrder RB) :
+    (A * B) -> (A * B) -> Prop :=
+    | prod_le_l
+        a0 a1 b0 b1
+        (ORD: RA a0 a1)
+        (NEQ: a0 <> a1)
+      :
+      prod_le PRA PRB (a0, b0) (a1, b1)
+    | prod_le_r
+        a b0 b1
+        (ORD: RB b0 b1)
+      :
+      prod_le PRA PRB (a, b0) (a, b1)
+  .
+
+  Global Program Instance prod_le_PreOrder
+         {A B: Type} {RA: A -> A -> Prop} {RB: B -> B -> Prop}
+         (PRA: PartialOrder RA) (PRB: PreOrder RB)
+    : PreOrder (prod_le PRA PRB).
+  Next Obligation.
+    ii. destruct x. econs 2. inv PRB. auto.
+  Qed.
+  Next Obligation.
+    ii. destruct x as [a0 b0], y as [a1 b1], z as [a2 b2].
+    inv H.
+    - inv H0.
+      + econs 1; inv PRA.
+        * inv partial_order_pre. eapply PreOrder_Transitive; eauto.
+        * ii. clarify. apply NEQ0. apply partial_order_anti_symm; auto.
+      + econs 1; auto.
+    - inv H0.
+      + econs 1; auto.
+      + econs 2. inv PRB. eapply PreOrder_Transitive; eauto.
+  Qed.
+
+End AUX.
+
+Module Tkst.
+  Section TKST.
+
+    Definition t X := (nat * X)%type.
+
+    Definition le {X} (s0 s1: @t X): Prop :=
+      let '(n0, x0) := s0 in
+      let '(n1, x1) := s1 in
+      (n0 <= n1) /\ (n0 = n1 -> x0 = x1).
+
+    Global Program Instance le_PreOrder X: PreOrder (@le X).
+    Next Obligation.
+      ii. unfold le. des_ifs.
+    Qed.
+    Next Obligation.
+      ii. unfold le in *. des_ifs. des; clarify. split; auto; try lia.
+      i. clarify. assert (n0 = n1). lia. clarify. rewrite H2; auto.
+    Qed.
+
+
+    Definition a {X} x : t X := (1, x).
+    Definition b {X} x : t X := (2, x).
+    Definition c {X} x : t X := (3, x).
+    Definition d {X} x : t X := (4, x).
+
+  End TKST.
+End Tkst.
+
+Section TKQ.
+
+  Inductive tkqueue
+            (l: list thread_id) (tks: NatMap.t TicketLockW.tk) (inc exc: TicketLockW.tk)
+    : Prop :=
+  | tkqueue_nil
+      (EMP1: l = [])
+      (EMP2: tks = @NatMap.empty _)
+      (EQ: inc = exc)
+    :
+    tkqueue l tks inc exc
+  | tkqueue_cons
+      hd tl
+      (QUEUE: l = hd :: tl)
+      (FIND: NatMap.find hd tks = Some inc)
+      (TL: tkqueue tl (NatMap.remove hd tks) (S inc) exc)
+    :
+    tkqueue l tks inc exc
+  .
+
+  Lemma tkqueue_enqueue
+        l tks inc exc
+        (TQ: tkqueue l tks inc exc)
+        k
+        (FIND: NatMap.find k tks = None)
+    :
+    tkqueue (l ++ [k]) (NatMap.add k exc tks) inc (S exc).
+  Proof.
+    revert_until TQ. induction TQ; i; clarify; ss.
+    { econs 2. ss. apply nm_find_add_eq. econs 1; auto. rewrite nm_find_none_rm_add_eq; auto. }
+    assert (NEQ: hd <> k).
+    { ii. clarify. }
+    econs 2. instantiate (2:=hd). ss. rewrite nm_find_add_neq; auto.
+    erewrite <- nm_find_none_add_rm_is_eq. eapply IHTQ.
+    rewrite nm_find_rm_neq; auto. rewrite nm_find_add_neq; auto. apply nm_find_rm_eq.
+    instantiate (1:=inc). rewrite nm_add_rm_comm_eq; auto.
+    rewrite <- nm_find_some_rm_add_eq; auto. rewrite nm_find_add_neq; auto.
+  Qed.
+
+  Lemma tkqueue_dequeue
+        l tks inc exc
+        (TQ: tkqueue l tks inc exc)
+        hd tl
+        (HD: l = hd :: tl)
+    :
+    tkqueue tl (NatMap.remove hd tks) (S inc) exc.
+  Proof.
+    revert_until TQ. induction TQ; i; clarify; ss.
+  Qed.
+
+  Lemma tkqueue_range
+        l tks inc exc
+        (TQ: tkqueue l tks inc exc)
+    :
+    inc <= exc.
+  Proof.
+    induction TQ; i; clarify; ss. lia.
+  Qed.
+
+  Lemma tkqueue_val_range_l
+        l tks inc exc
+        (TQ: tkqueue l tks inc exc)
+        t v
+        (FIND: NatMap.find t tks = Some v)
+    :
+    inc <= v.
+  Proof.
+    revert_until TQ. induction TQ; i; clarify; ss.
+    destruct (tid_dec t hd) eqn:DEC; clarify.
+    hexploit (IHTQ t v). rewrite nm_find_rm_neq; auto. i. lia.
+  Qed.
+
+  Lemma tkqueue_val_range_r
+        l tks inc exc
+        (TQ: tkqueue l tks inc exc)
+        t v
+        (FIND: NatMap.find t tks = Some v)
+    :
+    v < exc.
+  Proof.
+    revert_until TQ. induction TQ; i; clarify; ss.
+    destruct (tid_dec t hd) eqn:DEC; clarify.
+    - eapply tkqueue_range in TQ. lia.
+    - hexploit (IHTQ t v). rewrite nm_find_rm_neq; auto. i. lia.
+  Qed.
+
+  Lemma tkqueue_inv_unique
+        l tks inc exc
+        (TQ: tkqueue l tks inc exc)
+        t0 t1 v
+        (FIND0: NatMap.find t0 tks = Some v)
+        (FIND1: NatMap.find t1 tks = Some v)
+    :
+    t0 = t1.
+  Proof.
+    revert_until TQ. induction TQ; i; clarify; ss.
+    destruct (tid_dec t0 hd) eqn:DEC0; clarify; eauto.
+    { destruct (tid_dec t1 hd) eqn:DEC1; clarify; eauto.
+      hexploit tkqueue_val_range_l. eapply TQ. erewrite nm_find_rm_neq.
+      2:{ ii. apply n. symmetry. eapply H. }
+      eapply FIND1. i. lia.
+    }
+    { destruct (tid_dec t1 hd) eqn:DEC1; clarify; eauto.
+      { hexploit tkqueue_val_range_l. eapply TQ. erewrite nm_find_rm_neq.
+        2:{ ii. apply n. symmetry. eapply H. }
+        eapply FIND0. i. lia.
+      }
+      eapply IHTQ; rewrite nm_find_rm_neq; eauto.
+    }
+  Qed.
+
+  Lemma tkqueue_inv_hd
+        l tks inc exc
+        (TQ: tkqueue l tks inc exc)
+        t
+        (FIND: NatMap.find t tks = Some inc)
+    :
+    exists tl, l = t :: tl.
+  Proof.
+    revert_until TQ. induction TQ; i; clarify; ss.
+    destruct (tid_dec t hd) eqn:DEC; clarify; eauto.
+    hexploit tkqueue_inv_unique. 2: eapply FIND. 2: eapply FIND0.
+    { instantiate (1:=exc). instantiate (1:=inc). instantiate (1:=hd :: tl).
+      econs 2; eauto.
+    }
+    i; clarify.
+  Qed.
+
+  Lemma tkqueue_find_in
+        l tks inc exc
+        (TQ: tkqueue l tks inc exc)
+        t v
+        (FIND: NatMap.find t tks = Some v)
+    :
+    In t l.
+  Proof.
+    revert_until TQ. induction TQ; i; clarify; ss.
+    destruct (tid_dec t hd) eqn:DEC; clarify; auto.
+    right. hexploit (IHTQ t v). rewrite nm_find_rm_neq; auto. i. auto.
+  Qed.
+
+  Lemma tkqueue_in_find
+        l tks inc exc
+        (TQ: tkqueue l tks inc exc)
+        t
+        (IN: In t l)
+    :
+    exists v, NatMap.find t tks = Some v.
+  Proof.
+    revert_until TQ. induction TQ; i; clarify; ss. des; clarify; eauto.
+    hexploit (IHTQ t IN). i. des. exists v. rewrite NatMapP.F.remove_o in H. des_ifs.
+  Qed.
+
+End TKQ.
+
 Section SIM.
+
+  Context `{Σ: GRA.t}.
+
+  Context `{MONORA: @GRA.inG monoRA Σ}.
+  Context `{THDRA: @GRA.inG ThreadRA Σ}.
+  Context `{STATESRC: @GRA.inG (stateSrcRA (Mod.state AbsLock.mod)) Σ}.
+  Context `{STATETGT: @GRA.inG (stateTgtRA (OMod.closed_state TicketLockW.omod (WMem.mod))) Σ}.
+  Context `{IDENTSRC: @GRA.inG (identSrcRA (Mod.ident AbsLock.mod)) Σ}.
+  Context `{IDENTTGT: @GRA.inG (identTgtRA (OMod.closed_ident TicketLockW.omod (WMem.mod))) Σ}.
+  Context `{OBLGRA: @GRA.inG ObligationRA.t Σ}.
+  Context `{ARROWRA: @GRA.inG (ArrowRA (OMod.closed_ident TicketLockW.omod (WMem.mod))) Σ}.
+  Context `{EDGERA: @GRA.inG EdgeRA Σ}.
+  Context `{ONESHOTSRA: @GRA.inG (@FiniteMap.t (OneShot.t unit)) Σ}.
+  Context `{WMEMRA: @GRA.inG wmemRA Σ}.
+
+  Context `{NATMAPRA: @GRA.inG (Auth.t (NatMapRA.t TicketLockW.tk)) Σ}.
+  Context `{AUTHRA1: @GRA.inG (Auth.t (Excl.t nat)) Σ}.
+  Context `{AUTHRA2: @GRA.inG (Auth.t (Excl.t (nat * nat))) Σ}.
+  Context `{IN2: @GRA.inG (thread_id ==> (Auth.t (Excl.t nat)))%ra Σ}.
+
+  Let mypreord := prod_le_PreOrder nat_le_po (Tkst.le_PreOrder nat).
+  Variable monok: nat.
+  Variable tk_mono: nat.
+
+  Definition ticket_lock_inv_unlocking
+             (l: list thread_id) (tks: NatMap.t nat) (now next: nat) (myt: thread_id) : iProp :=
+    (own_thread myt)
+      ∗
+      (⌜tkqueue l tks (S now) next⌝)
+      ∗
+      (natmap_prop_sum tks (fun th tk => FairRA.white th (Ord.from_nat (tk - (S now)))))
+      ∗
+      (list_prop_sum (fun th => ((ObligationRA.duty (inl th) [])
+                                ∗ (∃ u, maps_to th (Auth.black (Excl.just u: Excl.t nat))))%I) l)
+      ∗
+      (∃ (k: nat) (o: Ord.t),
+          (monoBlack monok mypreord (now, Tkst.d k))
+            ∗ (ObligationRA.black k o)
+            ∗ (ObligationRA.pending k 1)
+            ∗ (ObligationRA.duty (inl myt) [(k, Ord.S Ord.O)])
+      )
+  .
+
+  Definition ticket_lock_inv_unlocked0
+             (l: list thread_id) (tks: NatMap.t nat) (now next: nat) (myt: thread_id) : iProp :=
+    (OwnM (Auth.white (Excl.just (now, myt): Excl.t (nat * nat)%type)))
+      ∗
+      (⌜(l = []) /\ (tks = @NatMap.empty _) /\ (now = next)⌝)
+      ∗
+      (∃ (k: nat),
+          (monoBlack monok mypreord (now, Tkst.a k))
+      )
+  .
+
+  Definition ticket_lock_inv_unlocked1
+             (l: list thread_id) (tks: NatMap.t nat) (now next: nat) (myt: thread_id) : iProp :=
+    ∃ yourt waits,
+      (OwnM (Auth.white (Excl.just (now, myt): Excl.t (nat * nat)%type)))
+        ∗
+        (⌜(l = yourt :: waits)⌝)
+        ∗
+        (⌜tkqueue l tks now next⌝)
+        ∗
+        (natmap_prop_sum tks (fun th tk => FairRA.white th (Ord.from_nat (tk - (now)))))
+        ∗
+        (list_prop_sum (fun th => ((ObligationRA.duty (inl th) [])
+                                  ∗ (∃ u, maps_to th (Auth.black (Excl.just u: Excl.t nat))))%I) waits)
+        ∗
+        (∃ (k: nat) (o: Ord.t) (u: nat),
+            (monoBlack monok mypreord (now, Tkst.b k))
+              ∗ (ObligationRA.black k o)
+              ∗ (ObligationRA.pending k 1)
+              ∗ (ObligationRA.duty (inl yourt) [(k, Ord.S Ord.O)])
+              ∗ (ObligationRA.white k (((Ord.S Ord.O) × Ord.omega) × (Ord.from_nat u))%ord)
+              ∗ (maps_to yourt (Auth.black (Excl.just u: Excl.t nat)))
+        )
+  .
+
+  Definition ticket_lock_inv_locked
+             (l: list thread_id) (tks: NatMap.t nat) (now next: nat) (myt: thread_id) : iProp :=
+    (OwnM (Auth.white (Excl.just (now, myt): Excl.t (nat * nat)%type)))
+      ∗
+      (⌜tkqueue l tks (S now) next⌝)
+      ∗
+      (natmap_prop_sum tks (fun th tk => FairRA.white th (Ord.from_nat (tk - (S now)))))
+      ∗
+      (list_prop_sum (fun th => ((ObligationRA.duty (inl th) [])
+                                ∗ (∃ u, maps_to th (Auth.black (Excl.just u: Excl.t nat))))%I) l)
+      ∗
+      (∃ (k: nat),
+          (monoBlack monok mypreord (now, Tkst.c k))
+      )
+  .
+
+  Definition ticket_lock_inv_tks
+             (tks: NatMap.t nat) : iProp :=
+    ((OwnM (Auth.black (Some tks: NatMapRA.t nat)))
+       ∗ (FairRA.whites (fun id => (~ NatMap.In id tks)) Ord.omega)
+       ∗ (natmap_prop_sum tks (fun tid tk => (own_thread tid)))
+       ∗ (OwnMs (fun id => (~ NatMap.In id tks))
+                ((Auth.black (Excl.just 0: Excl.t nat)) ⋅ (Auth.white (Excl.just 0: Excl.t nat))))
+    )
+  .
+
+  Definition ticket_lock_inv_mem
+             (mem: SCMem.t) (now next: nat) (myt: thread_id) : iProp :=
+    ((memory_black mem)
+       ∗ (points_to TicketLock.now_serving (SCMem.val_nat now))
+       ∗ (points_to TicketLock.next_ticket (SCMem.val_nat next))
+       ∗ (OwnM (Auth.black (Excl.just (now, myt): Excl.t (nat * nat)%type)))
+       ∗ (monoBlack tk_mono Nat.le_preorder now)
+    )
+  .
+
+  Definition ticket_lock_inv_state
+             (mem: SCMem.t) (own: bool) (tks: NatMap.t nat) : iProp :=
+    ((St_tgt (tt, mem)) ∗ (St_src (own, (key_set tks))))
+  .
+
+  Definition ticket_lock_inv : iProp :=
+    ∃ (mem: SCMem.t) (own: bool)
+      (l: list thread_id) (tks: NatMap.t nat) (now next: nat) (myt: thread_id),
+      (ticket_lock_inv_tks tks)
+        ∗
+        (ticket_lock_inv_mem mem now next myt)
+        ∗
+        (ticket_lock_inv_state mem own tks)
+        ∗
+        (((⌜own = true⌝)
+            ∗ (ticket_lock_inv_locked l tks now next myt)
+         )
+         ∨
+           ((⌜own = false⌝)
+              ∗ ((ticket_lock_inv_unlocking l tks now next myt)
+                 ∨
+                   ((ticket_lock_inv_unlocked0 l tks now next myt)
+                    ∨
+                      (ticket_lock_inv_unlocked1 l tks now next myt))
+                )
+        ))
+  .
+
+  Let I: list iProp := [ticket_lock_inv].
+
+  (* Properties *)
+  Lemma unlocking_mono
+        l tks now next myt:
+    (ticket_lock_inv_unlocking l tks now next myt)
+      -∗
+      ((⌜tkqueue l tks (S now) next⌝)
+         ∗
+         (∃ k o, (monoWhite monok mypreord (now, Tkst.d k))
+                   ∗ (ObligationRA.black k o)
+      )).
+  Proof.
+    iIntros "I". iDestruct "I" as "[_ [%I2 [_ [_ I]]]]". do 2 iDestruct "I" as "[% I]".
+    iDestruct "I" as "[MB [OB _]]". iPoseProof (black_white with "MB") as "#MYTURN".
+    iSplit. auto. iExists k, o. iFrame. auto.
+  Qed.
+
+  Lemma unlocking_contra
+        tid l tks now next myt
+        (FIND: NatMap.find tid tks = Some now)
+    :
+    (ticket_lock_inv_unlocking l tks now next myt)
+      -∗ ⌜False⌝.
+  Proof.
+    iIntros "I". iDestruct "I" as "[_ [%I2 [_ [_ _]]]]". exfalso.
+    hexploit (tkqueue_val_range_l I2 _ FIND). i. lia.
+  Qed.
+
+  Lemma unlocking_myturn
+        tid l tks now next myt
+        mytk o
+        (FIND: NatMap.find tid tks = Some mytk)
+    :
+    (monoWhite monok mypreord (mytk, o))
+      -∗
+      (ticket_lock_inv_unlocking l tks now next myt)
+      -∗ ⌜False⌝.
+  Proof.
+    iIntros "MYT I". iDestruct "I" as "[_ [%I2 [_ [_ I3]]]]".
+    do 2 (iDestruct "I3" as "[% I3]"). iDestruct "I3" as "[I3 _]".
+    iPoseProof (black_white_compare with "MYT I3") as "%LE". exfalso.
+    hexploit (tkqueue_val_range_l I2 _ FIND). i. inv LE; try lia.
+  Qed.
+
+  Lemma unlocked0_contra
+        tid l tks now next myt mytk
+        (FIND: NatMap.find tid tks = Some mytk)
+    :
+    (ticket_lock_inv_unlocked0 l tks now next myt)
+      -∗ ⌜False⌝.
+  Proof.
+    iIntros "I". iDestruct "I" as "[_ [%I2 _]]". exfalso. des; clarify.
+  Qed.
+
+  Lemma unlocked1_mono
+        l tks now next myt:
+    (ticket_lock_inv_unlocked1 l tks now next myt)
+      -∗
+      ((⌜tkqueue l tks now next⌝)
+         ∗
+         (∃ k o, (monoWhite monok mypreord (now, Tkst.b k))
+                   ∗ (ObligationRA.black k o)
+      )).
+  Proof.
+    iIntros "I". do 2 iDestruct "I" as "[% I]". iDestruct "I" as "[_ [_ [%I3 [_ [_ I]]]]]".
+    do 3 iDestruct "I" as "[% I]". iDestruct "I" as "[MB [OB _]]".
+    iSplit. auto. iPoseProof (black_white with "MB") as "#MYTURN". iExists k, o. iFrame. auto.
+  Qed.
+
+  Lemma unlocked1_myturn
+        tid l tks now next myt
+        mytk o
+        (FIND: NatMap.find tid tks = Some mytk)
+    :
+    (monoWhite monok mypreord (mytk, o))
+      -∗
+      (ticket_lock_inv_unlocked1 l tks now next myt)
+      -∗ ⌜now = mytk⌝.
+  Proof.
+    iIntros "MYT I". do 2 iDestruct "I" as "[% I]". iDestruct "I" as "[_ [%I1 [%I2 [_ [_ I]]]]]".
+    do 3 iDestruct "I" as "[% I]". iDestruct "I" as "[MB _]".
+    iPoseProof (black_white_compare with "MYT MB") as "%LE".
+    hexploit (tkqueue_val_range_l I2 _ FIND). i. inv LE; auto. lia.
+  Qed.
+
+  Lemma locked_contra
+        tid l tks now next myt
+        (FIND: NatMap.find tid tks = Some now)
+    :
+    (ticket_lock_inv_locked l tks now next myt)
+      -∗ ⌜False⌝.
+  Proof.
+    iIntros "I". iDestruct "I" as "[_ [%I2 _]]". exfalso.
+    hexploit (tkqueue_val_range_l I2 _ FIND). clear. i. lia.
+  Qed.
+
+  Lemma locked_myturn
+        tid l tks now next myt
+        mytk o
+        (FIND: NatMap.find tid tks = Some mytk)
+    :
+    (monoWhite monok mypreord (mytk, o))
+      -∗
+      (ticket_lock_inv_locked l tks now next myt)
+      -∗ ⌜False⌝.
+  Proof.
+    iIntros "MYT I". iDestruct "I" as "[_ [%I2 [_ [_ [% I3]]]]]".
+    iPoseProof (black_white_compare with "MYT I3") as "%LE". exfalso.
+    hexploit (tkqueue_val_range_l I2 _ FIND). i. inv LE; try lia.
+  Qed.
+
+  Lemma mytk_find_some tid mytk tks:
+    (OwnM (Auth.white (NatMapRA.singleton tid mytk: NatMapRA.t nat)))
+      ∗ (ticket_lock_inv_tks tks)
+      -∗ ⌜NatMap.find tid tks = Some mytk⌝.
+  Proof.
+    iIntros "[MYTK TKS]". iDestruct "TKS" as "[TKS0 _]".
+    iApply (NatMapRA_find_some with "TKS0 MYTK").
+  Qed.
+
+  Lemma ticket_lock_inv_mem_mono
+        mem now next myt
+    :
+    (ticket_lock_inv_mem mem now next myt)
+      -∗
+      (monoWhite tk_mono Nat.le_preorder now).
+  Proof.
+    iIntros "MEM". iDestruct "MEM" as "[MEM0 [MEM1 [MEM2 [MEM3 MEM4]]]]".
+    iPoseProof (black_white with "MEM4") as "#MONOTK".
+    auto.
+  Qed.
+
+  (* Simulations *)
+  Lemma lock_enqueue tid:
+    ((own_thread tid)
+       ∗ (ObligationRA.duty (inl tid) [])
+    )
+      ∗
+      (∀ mytk,
+          (
+            (OwnM (Auth.white (NatMapRA.singleton tid mytk: NatMapRA.t TicketLockW.tk)))
+              ∗ (maps_to tid (Auth.white (Excl.just 2: Excl.t nat)))
+          )
+          -∗
+  (stsim I tid (topset I) ibot7 ibot7
+         (λ r_src r_tgt : (), (own_thread tid ** ObligationRA.duty (inl tid) []) ** ⌜r_src = r_tgt⌝)
+         false false
+    (ITree.iter
+        (λ _ : (),
+           trigger Yield;;;
+           ` x_0 : bool * NatMap.t () <- trigger (Get (bool * NatMap.t ()));;
+           (let (own0, _) := x_0 in if Bool.eqb own0 true then Ret (inl ()) else Ret (inr ())))
+        ();;;
+      ` x_0 : bool * NatMap.t () <- trigger (Get (bool * NatMap.t ()));;
+      (let (_, ts0) := x_0 in
+       trigger (Put (true, NatMap.remove (elt:=()) tid ts0));;;
+       trigger
+         (Fair
+            (λ i : nat,
+               if tid_dec i tid
+               then Flag.success
+               else
+                if NatMapP.F.In_dec (NatMap.remove (elt:=()) tid ts0) i
+                then Flag.fail
+                else Flag.emp));;; trigger Yield;;; Ret ()))
+    (OMod.close_itree TicketLock.omod (SCMem.mod TicketLock.gvs)
+       (TicketLock.lock_loop (SCMem.val_nat mytk));;;
+     OMod.close_itree TicketLock.omod (SCMem.mod TicketLock.gvs) (trigger Yield))
+  )
+      )
+      ⊢
+      (stsim I tid (topset I) ibot7 ibot7
+             (fun r_src r_tgt => own_thread tid ** ObligationRA.duty (inl tid) [] ** ⌜r_src = r_tgt⌝)
+             false false
+             (AbsLock.lock_fun tt)
+             (OMod.close_itree TicketLock.omod (SCMem.mod TicketLock.gvs)
+                               (TicketLock.lock_fun tt))).
+  Proof.
+    iIntros "[[MYTH DUTY] SIM]".
+    unfold AbsLock.lock_fun, TicketLock.lock_fun. rred.
+    rewrite close_itree_call. rred.
+    iApply (stsim_sync with "[DUTY]"). msubtac. iFrame. iIntros "DUTY _".
+    unfold Mod.wrap_fun, SCMem.faa_fun. rred.
+    iApply stsim_tidL. lred.
+
+    iopen 0 "I" "K". do 7 iDestruct "I" as "[% I]". iDestruct "I" as "[TKS [MEM [ST CASES]]]".
+    iDestruct "ST" as "[ST0 ST1]".
+    iApply stsim_getL. iSplit. auto. iApply (stsim_putL with "ST1"). iIntros "ST1".
+
+    iApply stsim_getR. iSplit. auto. rred. iApply stsim_tauR. rred.
+    iDestruct "MEM" as "[MEM0 [MEM1 [MEM2 MEM3]]]".
+    iPoseProof (memory_ra_faa with "MEM0 MEM2") as "[% [%FAA >[MEM0 MEM2]]]".
+    erewrite FAA. rred.
+    iApply stsim_getR. iSplit. auto. rred.
+    iApply (stsim_putR with "ST0"). iIntros "ST0". rred.
+    iApply stsim_tauR. rred. iApply stsim_tauR. rred.
+
+    iAssert (⌜NatMap.find tid tks = None⌝)%I as "%FINDNONE".
+    { destruct (NatMap.find tid tks) eqn:FIND; auto.
+      iDestruct "TKS" as "[_ [_ [YTH _]]]". iPoseProof (natmap_prop_sum_in with "YTH") as "FALSE".
+      eauto. iPoseProof (own_thread_unique with "MYTH FALSE") as "%FALSE". auto.
+    }
+
+    iDestruct "TKS" as "[TKS0 [TKS1 [TKS2 TKS3]]]".
+    set (tks' := NatMap.add tid next tks).
+    iPoseProof (NatMapRA_add with "TKS0") as ">[TKS0 MYTK]". eauto. instantiate (1:=next).
+    iAssert (St_src (own, (key_set tks')))%I with "[ST1]" as "ST1".
+    { subst tks'. rewrite key_set_pull_add_eq. iFrame. }
+    iPoseProof ((FairRA.whites_unfold (fun id => ~ NatMap.In id tks') _ (i:=tid)) with "TKS1") as "[TKS1 MYTRI]".
+    { subst tks'. i. ss. des; clarify.
+      - ii. apply IN. destruct (tid_dec j tid); clarify.
+        apply NatMapP.F.not_find_in_iff in H; clarify. apply NatMapP.F.add_in_iff; auto.
+      - apply NatMapP.F.not_find_in_iff; auto.
+    }
+    { subst tks'. ii. apply H. apply NatMapP.F.add_in_iff. auto. }
+
+    iPoseProof ((OwnMs_unfold (fun id => ~ NatMap.In id tks') _ (i:=tid)) with "TKS3") as "[TKS3 MYNUM]".
+    { subst tks'. i. ss. des; clarify.
+      - ii. apply IN. destruct (tid_dec j tid); clarify.
+        apply NatMapP.F.not_find_in_iff in H; clarify. apply NatMapP.F.add_in_iff; auto.
+      - apply NatMapP.F.not_find_in_iff; auto.
+    }
+    { subst tks'. ii. apply H. apply NatMapP.F.add_in_iff. auto. }
+    iPoseProof (OwnM_Upd with "MYNUM") as "> MYNUM".
+    { eapply maps_to_updatable. apply Auth.auth_update.
+      instantiate (1:=Excl.just 2). instantiate (1:=Excl.just 2).
+      ii. des. ur in FRAME. des_ifs. split.
+      { ur. ss. }
+      { ur. ss. }
+    }
+    rewrite <- maps_to_res_add. iDestruct "MYNUM" as "[MYNB MYNW]".
+
+    iAssert (natmap_prop_sum tks' (λ tid0 _ : nat, own_thread tid0))%I with "[MYTH TKS2]" as "TKS2".
+    { subst tks'. iApply (natmap_prop_sum_add with "TKS2"). iFrame. }
+
+    iDestruct "CASES" as "[[%TRUE INV] | [%FALSE INV]]"; subst.
+    { iPoseProof (FairRA.white_mon with "MYTRI") as ">MYTRI".
+      { instantiate (1:=Ord.from_nat (next - (S now))). ss.
+        apply Ord.lt_le. apply Ord.omega_upperbound.
+      }
+      iMod ("K" with "[DUTY TKS0 TKS1 TKS2 TKS3 MEM0 MEM1 MEM2 MEM3 INV ST0 ST1 MYTRI MYNB]") as "_".
+      { subst tks'. unfold ticket_lock_inv.
+        iExists m1, true, (l ++ [tid]), (NatMap.add tid next tks), now, (S next), myt.
+        iFrame.
+        iSplitL "MEM2".
+        { ss. replace (S next) with (next + 1). iFrame. lia. }
+        iLeft. iSplit; auto. unfold ticket_lock_inv_locked.
+        iDestruct "INV" as "[INV0 [INV1 [INV2 [INV3 INV4]]]]". iFrame.
+        iSplit.
+        { iPure "INV1" as ?. iPureIntro. apply tkqueue_enqueue; auto. }
+        iPoseProof (natmap_prop_sum_add with "INV2 MYTRI") as "INV2". iFrame.
+        iApply list_prop_sum_add. iFrame. iExists 2. iFrame.
+      }
+      iApply stsim_reset. iApply "SIM". iFrame.
+    }
+
+    iDestruct "INV" as "[INV | INV]".
+    { iPoseProof (FairRA.white_mon with "MYTRI") as ">MYTRI".
+      { instantiate (1:=Ord.from_nat (next - (S now))). ss.
+        apply Ord.lt_le. apply Ord.omega_upperbound.
+      }
+      iMod ("K" with "[DUTY TKS0 TKS1 TKS2 TKS3 MEM0 MEM1 MEM2 MEM3 INV ST0 ST1 MYTRI MYNB]") as "_".
+      { subst tks'. unfold ticket_lock_inv.
+        iExists m1, false, (l ++ [tid]), (NatMap.add tid next tks), now, (S next), myt.
+    remember ((⌜false = true⌝ **
+     ticket_lock_inv_locked (l ++ [tid]) (NatMap.add tid next tks) now (S next) myt)
+    ∨ (⌜false = false⌝ **
+       ticket_lock_inv_unlocking (l ++ [tid]) (NatMap.add tid next tks) now (S next) myt
+       ∨ ticket_lock_inv_unlocked0 (l ++ [tid]) (NatMap.add tid next tks) now (S next) myt
+         ∨ ticket_lock_inv_unlocked1 (l ++ [tid]) (NatMap.add tid next tks) now (S next) myt))%I as temp.
+        iFrame. subst temp.
+        iSplitL "MEM2".
+        { ss. replace (S next) with (next + 1). iFrame. lia. }
+        iRight. iSplit; auto. iLeft. unfold ticket_lock_inv_unlocking.
+        iDestruct "INV" as "[INV0 [INV1 [INV2 [INV3 INV4]]]]". iFrame.
+        iSplit.
+        { iPure "INV1" as ?. iPureIntro. apply tkqueue_enqueue; auto. }
+        iPoseProof (natmap_prop_sum_add with "INV2 MYTRI") as "INV2". iFrame.
+        iApply list_prop_sum_add. iFrame. iExists 2. iFrame.
+      }
+      iApply stsim_reset. iApply "SIM". iFrame.
+    }
+
+    iDestruct "INV" as "[INV | INV]".
+    { iPoseProof (FairRA.white_mon with "MYTRI") as ">MYTRI".
+      { instantiate (1:=Ord.from_nat (next - (now))). ss.
+        apply Ord.lt_le. apply Ord.omega_upperbound.
+      }
+      iPoseProof (ObligationRA.alloc (((Ord.S Ord.O) × Ord.omega) × (Ord.from_nat 3))%ord) as "> [% [[OBLK OWHI] OPEND]]".
+      iPoseProof (ObligationRA.white_eq with "OWHI") as "OWHI".
+      { rewrite Ord.from_nat_S. rewrite Jacobsthal.mult_S. reflexivity. }
+      iPoseProof (ObligationRA.white_split_eq with "OWHI") as "[OWHI TAX]".
+      iPoseProof (ObligationRA.duty_alloc with "DUTY OWHI") as "> DUTY".
+      unfold ticket_lock_inv_unlocked0. iDestruct "INV" as "[INV0 [% [% INV2]]]".
+      iPoseProof ((black_updatable _ _ _ (now, Tkst.b k)) with "INV2") as ">INV2".
+      { econs 2. ss. split; auto. i; ss. }
+
+      iMod ("K" with "[DUTY TKS0 TKS1 TKS2 TKS3 MEM0 MEM1 MEM2 MEM3 INV0 INV2 ST0 ST1 MYTRI MYNB OBLK OPEND TAX]") as "_".
+      { subst tks'. unfold ticket_lock_inv.
+        iExists m1, false, (l ++ [tid]), (NatMap.add tid next tks), now, (S next), myt.
+    remember ((⌜false = true⌝ **
+     ticket_lock_inv_locked (l ++ [tid]) (NatMap.add tid next tks) now (S next) myt)
+    ∨ (⌜false = false⌝ **
+       ticket_lock_inv_unlocking (l ++ [tid]) (NatMap.add tid next tks) now (S next) myt
+       ∨ ticket_lock_inv_unlocked0 (l ++ [tid]) (NatMap.add tid next tks) now (S next) myt
+         ∨ ticket_lock_inv_unlocked1 (l ++ [tid]) (NatMap.add tid next tks) now (S next) myt))%I as temp.
+        iFrame. subst temp.
+        iSplitL "MEM2".
+        { ss. replace (S next) with (next + 1). iFrame. lia. }
+        iRight. iSplit; auto. iRight. iRight.
+        unfold ticket_lock_inv_unlocked1.
+        des; clarify. ss. iExists tid, []. ss. iFrame.
+        iSplit; auto.
+        iSplit.
+        { iPureIntro. econs 2; eauto. apply NatMapP.F.add_eq_o; auto. econs 1; auto.
+          apply nm_find_none_rm_add_eq. apply NatMapP.F.empty_o.
+        }
+        iSplitR. auto. iExists k, _, 2. iFrame.
+      }
+      iApply stsim_reset. iApply "SIM". iFrame.
+    }
+
+    { iPoseProof (FairRA.white_mon with "MYTRI") as ">MYTRI".
+      { instantiate (1:=Ord.from_nat (next - (now))). ss.
+        apply Ord.lt_le. apply Ord.omega_upperbound.
+      }
+      iMod ("K" with "[DUTY TKS0 TKS1 TKS2 TKS3 MEM0 MEM1 MEM2 MEM3 INV ST0 ST1 MYTRI MYNB]") as "_".
+      { subst tks'. unfold ticket_lock_inv.
+        iExists m1, false, (l ++ [tid]), (NatMap.add tid next tks), now, (S next), myt.
+    remember ((⌜false = true⌝ **
+     ticket_lock_inv_locked (l ++ [tid]) (NatMap.add tid next tks) now (S next) myt)
+    ∨ (⌜false = false⌝ **
+       ticket_lock_inv_unlocking (l ++ [tid]) (NatMap.add tid next tks) now (S next) myt
+       ∨ ticket_lock_inv_unlocked0 (l ++ [tid]) (NatMap.add tid next tks) now (S next) myt
+         ∨ ticket_lock_inv_unlocked1 (l ++ [tid]) (NatMap.add tid next tks) now (S next) myt))%I as temp.
+        iFrame. subst temp.
+        iSplitL "MEM2".
+        { ss. replace (S next) with (next + 1). iFrame. lia. }
+        iRight. iSplit; auto. iRight. iRight. unfold ticket_lock_inv_unlocked1.
+        do 2 iDestruct "INV" as "[% INV]".
+        iDestruct "INV" as "[INV0 [% [INV2 [INV3 [INV4 INV5]]]]]". subst.
+        iExists yourt, (waits ++ [tid]). ss. iFrame.
+        iSplit. auto.
+        iSplit.
+        { iPure "INV2" as ?. iPureIntro. rewrite app_comm_cons. apply tkqueue_enqueue; auto. }
+        iPoseProof (natmap_prop_sum_add with "INV3 MYTRI") as "INV3". iFrame.
+        iApply list_prop_sum_add. iFrame. iExists 2. iFrame.
+      }
+      iApply stsim_reset. iApply "SIM". iFrame.
+    }
+  Qed.
+
+  Lemma lock_myturn_yieldR
+        (g0 g1 : ∀ R_src R_tgt : Type,
+            (R_src → R_tgt → iProp)
+            → bool
+            → bool
+            → itree ((eventE +' cE) +' sE (Mod.state AbsLock.mod)) R_src
+            → itree
+                ((eventE +' cE) +'
+                                   sE (OMod.closed_state TicketLock.omod (SCMem.mod TicketLock.gvs))) R_tgt
+            → iProp)
+        (ps pt: bool)
+        (src: itree ((eventE +' cE) +' sE (Mod.state AbsLock.mod)) unit)
+        (tgt: itree ((eventE +' cE) +' sE (OMod.closed_state TicketLock.omod (SCMem.mod TicketLock.gvs))) unit)
+        (tid mytk u: nat)
+        x
+    :
+    (
+      (OwnM (Auth.white ((NatMapRA.singleton tid mytk: NatMapRA.t TicketLockW.tk))))
+        ∗ (maps_to tid (Auth.white (Excl.just (S u): Excl.t nat)))
+        ∗ (monoWhite monok mypreord (mytk, x))
+    )
+      ∗
+      (
+      ((OwnM (Auth.white ((NatMapRA.singleton tid mytk: NatMapRA.t TicketLockW.tk))))
+        ∗ (maps_to tid (Auth.white (Excl.just u: Excl.t nat)))
+        ∗ (monoWhite monok mypreord (mytk, x)))
+        -∗
+  (stsim I tid (topset I) g0 g1
+    (λ r_src r_tgt : (), (own_thread tid ** ObligationRA.duty (inl tid) []) ** ⌜r_src = r_tgt⌝)
+    ps true
+    (trigger Yield;;; src)
+    (tgt))
+      )
+      ⊢
+  (stsim I tid (topset I) g0 g1
+    (λ r_src r_tgt : (), (own_thread tid ** ObligationRA.duty (inl tid) []) ** ⌜r_src = r_tgt⌝)
+    ps pt
+    (trigger Yield;;; src)
+    (trigger Yield;;; tgt)).
+  Proof.
+    iIntros "[[MYTK [MYNW MYTURN]] SIM]".
+    iopen 0 "I" "K". do 7 iDestruct "I" as "[% I]". iDestruct "I" as "[TKS [MEM [ST CASES]]]".
+    iPoseProof (mytk_find_some with "[MYTK TKS]") as "%FIND". iFrame.
+    iDestruct "CASES" as "[[%CT I] | [%CF [I | [I | I]]]]".
+    { iPoseProof (locked_myturn with "MYTURN I") as "%FF". eauto. inv FF. }
+    { iPoseProof (unlocking_myturn with "MYTURN I") as "%FF". eauto. inv FF. }
+    { iPoseProof (unlocked0_contra with "I") as "%FF". eauto. inv FF. }
+    iPoseProof (unlocked1_myturn with "MYTURN I") as "%EQ". eauto. subst mytk.
+    do 2 iDestruct "I" as "[% I]". iDestruct "I" as "[I0 [% [%I2 [I3 [I4 I5]]]]]".
+    do 3 iDestruct "I5" as "[% I5]". iDestruct "I5" as "[I5 I6]".
+    iDestruct "I6" as "[I6 [I7 [I8 [I9 I10]]]]".
+    hexploit (tkqueue_inv_hd I2 _ FIND). i. des.
+    inv H. symmetry in H1. inv H1.
+
+    iCombine "I10 MYNW" as "MYNUM".
+    iPoseProof (OwnM_valid with "MYNUM") as "%EQ".
+    assert (u0 = S u).
+    { clear -EQ. ur in EQ. specialize (EQ tid). unfold maps_to_res in EQ.
+      des_ifs. ur in EQ. des. rr in EQ. des. ur in EQ. des_ifs.
+    }
+    subst u0. clear EQ.
+    iPoseProof (OwnM_Upd with "MYNUM") as "> MYNUM".
+    { rewrite maps_to_res_add. eapply maps_to_updatable. eapply Auth.auth_update.
+      instantiate (1:=Excl.just u). instantiate (1:=Excl.just u).
+      ii. des. ur in FRAME. des_ifs. split; ur; ss.
+    }
+    rewrite <- maps_to_res_add. iDestruct "MYNUM" as "[I10 MYNW]".
+
+    iPoseProof (ObligationRA.white_eq with "I9") as "I9".
+    { rewrite Ord.from_nat_S. rewrite Jacobsthal.mult_S. reflexivity. }
+    iPoseProof (ObligationRA.white_split_eq with "I9") as "[TAX I9]".
+    iApply (stsim_yieldR_strong with "[I8 TAX]").
+    { iFrame. iApply ObligationRA.tax_cons_fold. iFrame. }
+    iIntros "I8 _".
+    iMod ("K" with "[TKS MEM ST I0 I3 I4 I5 I6 I7 I8 I9 I10]") as "_".
+    { iExists mem, false, (tid :: tl), tks, now, next, myt.
+      remember (
+          (⌜false = true⌝ ** ticket_lock_inv_locked (tid :: tl) tks now next myt)
+          ∨ (⌜false = false⌝ **
+                           ticket_lock_inv_unlocking (tid :: tl) tks now next myt
+             ∨ ticket_lock_inv_unlocked0 (tid :: tl) tks now next myt
+             ∨ ticket_lock_inv_unlocked1 (tid :: tl) tks now next myt))%I as temp.
+      iFrame. subst temp.
+      iRight. iSplit. auto. iRight. iRight.
+      iExists tid, tl. iFrame. iSplit. auto. iSplit. auto.
+      iExists k, o, u. iFrame.
+    }
+    iModIntro. iApply "SIM". iFrame.
+  Qed.
+
+  Lemma lock_yourturn_yieldR
+        (g0 g1 : ∀ R_src R_tgt : Type,
+            (R_src → R_tgt → iProp)
+            → bool
+            → bool
+            → itree ((eventE +' cE) +' sE (Mod.state AbsLock.mod)) R_src
+            → itree
+                ((eventE +' cE) +'
+                                   sE (OMod.closed_state TicketLock.omod (SCMem.mod TicketLock.gvs))) R_tgt
+            → iProp)
+        (ps pt: bool)
+        (src: itree ((eventE +' cE) +' sE (Mod.state AbsLock.mod)) unit)
+        (tgt: itree ((eventE +' cE) +' sE (OMod.closed_state TicketLock.omod (SCMem.mod TicketLock.gvs))) unit)
+        (tid mytk now: nat)
+        tks mem next l myt own
+        (NEQ: mytk <> now)
+    :
+  (OwnM (Auth.white (NatMapRA.singleton tid mytk: NatMapRA.t nat)) **
+    (ticket_lock_inv_tks tks **
+     (ticket_lock_inv_mem mem now next myt **
+      (ticket_lock_inv_state mem own tks **
+       ((⌜own = true⌝ ** ticket_lock_inv_locked l tks now next myt)
+        ∨ (⌜own = false⌝ **
+           ticket_lock_inv_unlocking l tks now next myt
+           ∨ ticket_lock_inv_unlocked0 l tks now next myt
+             ∨ ticket_lock_inv_unlocked1 l tks now next myt) **
+        (ticket_lock_inv -*
+         MUpd (nth_default True%I I)
+           (fairI (ident_tgt:=OMod.closed_ident TicketLock.omod (SCMem.mod TicketLock.gvs))) []
+           [0] True))))))
+      ∗
+      (((OwnM (Auth.white ((NatMapRA.singleton tid mytk: NatMapRA.t nat))))
+          ∗ (FairRA.white_thread (_Id:=_)))
+        -∗
+  (stsim I tid (topset I) g0 g1
+    (λ r_src r_tgt : (), (own_thread tid ** ObligationRA.duty (inl tid) []) ** ⌜r_src = r_tgt⌝)
+    ps true
+    (trigger Yield;;; src)
+    (tgt))
+      )
+      ⊢
+  (stsim I tid [] g0 g1
+    (λ r_src r_tgt : (), (own_thread tid ** ObligationRA.duty (inl tid) []) ** ⌜r_src = r_tgt⌝)
+    ps pt
+    (trigger Yield;;; src)
+    (trigger Yield;;; tgt)).
+  Proof.
+    iIntros "[[MYTH [TKS [MEM [ST [CASES K]]]]] SIM]".
+    iPoseProof (mytk_find_some with "[MYTH TKS]") as "%FIND". iFrame.
+    iDestruct "CASES" as "[[CT INV]|[CF INV]]".
+    { unfold ticket_lock_inv_locked. iDestruct "INV" as "[INV0 [%INV1 [INV2 [INV3 INV4]]]]".
+      hexploit (tkqueue_find_in INV1 _ FIND). i.
+      iPoseProof (list_prop_sum_in_split with "INV3") as "[[DUTY MAPS] INV3]". eapply H.
+      iApply (stsim_yieldR_strong with "[DUTY]"). iFrame. iIntros "DUTY RIGHT".
+      iMod ("K" with "[TKS MEM ST CT INV0 INV2 INV4 MAPS INV3 DUTY]") as "_".
+      { iExists mem, own, l, tks, now, next, myt.
+        remember 
+    ((⌜own = true⌝ ** ticket_lock_inv_locked l tks now next myt)
+    ∨ (⌜own = false⌝ **
+       ticket_lock_inv_unlocking l tks now next myt
+       ∨ ticket_lock_inv_unlocked0 l tks now next myt
+       ∨ ticket_lock_inv_unlocked1 l tks now next myt))%I as temp. iFrame. subst temp.
+        iLeft. iSplit. auto. iFrame. iSplit. auto. iApply "INV3". iFrame.
+      }
+      iModIntro. iApply "SIM". iFrame.
+    }
+    iDestruct "INV" as "[INV | [INV | INV]]".
+    { iDestruct "INV" as "[INV0 [%INV1 [INV2 [INV3 INV4]]]]".
+      hexploit (tkqueue_find_in INV1 _ FIND). i.
+      iPoseProof (list_prop_sum_in_split with "INV3") as "[[DUTY MAPS] INV3]". eapply H.
+      iApply (stsim_yieldR_strong with "[DUTY]"). iFrame. iIntros "DUTY RIGHT".
+      iMod ("K" with "[TKS MEM ST CF INV0 INV2 INV4 MAPS INV3 DUTY]") as "_".
+      { iExists mem, own, l, tks, now, next, myt.
+        remember 
+    ((⌜own = true⌝ ** ticket_lock_inv_locked l tks now next myt)
+    ∨ (⌜own = false⌝ **
+       ticket_lock_inv_unlocking l tks now next myt
+       ∨ ticket_lock_inv_unlocked0 l tks now next myt
+       ∨ ticket_lock_inv_unlocked1 l tks now next myt))%I as temp. iFrame. subst temp.
+        iRight. iSplit. auto. iLeft. iFrame. iSplit. auto. iApply "INV3". iFrame.
+      }
+      iModIntro. iApply "SIM". iFrame.
+    }
+    { iDestruct "INV" as "[INV0 [%INV1 INV2]]". exfalso. des; clarify. }
+    { do 2 iDestruct "INV" as "[% INV]".
+      iDestruct "INV" as "[INV0 [%INV1 [%INV2 [INV3 [INV4 INV5]]]]]".
+      hexploit (tkqueue_dequeue INV2). eapply INV1. i.
+      assert (NOTMT: tid <> yourt).
+      { ii. clarify. inv INV2; ss. clarify. setoid_rewrite FIND in FIND0. inv FIND0. ss. }
+      hexploit (tkqueue_find_in H).
+      { instantiate (1:=mytk). instantiate (1:=tid). rewrite nm_find_rm_neq; auto. }
+      intro IN.
+      iPoseProof (list_prop_sum_in_split with "INV4") as "[[DUTY MAPS] INV4]". eapply IN.
+      iApply (stsim_yieldR_strong with "[DUTY]"). iFrame. iIntros "DUTY RIGHT".
+      iMod ("K" with "[TKS MEM ST CF INV0 INV3 INV5 MAPS INV4 DUTY]") as "_".
+      { iExists mem, own, l, tks, now, next, myt.
+        remember 
+    ((⌜own = true⌝ ** ticket_lock_inv_locked l tks now next myt)
+    ∨ (⌜own = false⌝ **
+       ticket_lock_inv_unlocking l tks now next myt
+       ∨ ticket_lock_inv_unlocked0 l tks now next myt
+       ∨ ticket_lock_inv_unlocked1 l tks now next myt))%I as temp. iFrame. subst temp.
+        iRight. iSplit. auto. iRight. iRight. iFrame. iExists yourt, waits.
+        iSplit. auto. iSplit. auto. iFrame. iApply "INV4". iFrame.
+      }
+      iModIntro. iApply "SIM". iFrame.
+    }
+  Qed.
+
+  Lemma lock_myturn0
+        (g0 g1 : ∀ R_src R_tgt : Type,
+            (R_src → R_tgt → iProp)
+            → bool
+            → bool
+            → itree ((eventE +' cE) +' sE (Mod.state AbsLock.mod)) R_src
+            → itree ((eventE +' cE) +' sE (OMod.closed_state TicketLock.omod (SCMem.mod TicketLock.gvs))) R_tgt → iProp)
+        (ps pt: bool)
+        (tid : nat)
+        (mytk : TicketLockW.tk)
+        x tx
+        (TX: 1 <= tx)
+    :
+    ((monoWhite monok mypreord (mytk, x))
+       ∗ (OwnM (Auth.white (NatMapRA.singleton tid mytk: NatMapRA.t nat)))
+       ∗ (maps_to tid (Auth.white (Excl.just tx: Excl.t nat))))
+  ⊢ stsim I tid (topset I) g0 g1
+      (λ r_src r_tgt : (), (own_thread tid ** ObligationRA.duty (inl tid) []) ** ⌜r_src = r_tgt⌝)
+      ps pt
+      (trigger Yield;;;
+       ` x : () + () <-
+       (` x_0 : bool * NatMap.t () <- trigger (Get (bool * NatMap.t ()));;
+        (let (own0, _) := x_0 in if Bool.eqb own0 true then Ret (inl ()) else Ret (inr ())));;
+       match x with
+       | inl l0 =>
+           tau;; ITree.iter
+                   (λ _ : (),
+                      trigger Yield;;;
+                      ` x_0 : bool * NatMap.t () <- trigger (Get (bool * NatMap.t ()));;
+                      (let (own0, _) := x_0 in
+                       if Bool.eqb own0 true then Ret (inl ()) else Ret (inr ()))) l0
+       | inr r0 => Ret r0
+       end;;;
+       ` x_0 : bool * NatMap.t () <- trigger (Get (bool * NatMap.t ()));;
+       (let (_, ts0) := x_0 in
+        trigger (Put (true, NatMap.remove (elt:=()) tid ts0));;;
+        trigger
+          (Fair
+             (λ i : nat,
+                if tid_dec i tid
+                then Flag.success
+                else
+                 if NatMapP.F.In_dec (NatMap.remove (elt:=()) tid ts0) i
+                 then Flag.fail
+                 else Flag.emp));;; trigger Yield;;; Ret ()))
+      (` r : Any.t <-
+       OMod.embed_itree TicketLock.omod (SCMem.mod TicketLock.gvs)
+         (Mod.wrap_fun SCMem.load_fun (Any.upcast TicketLock.now_serving));;
+       ` x : SCMem.val <- (tau;; unwrap (Any.downcast r));;
+       OMod.close_itree TicketLock.omod (SCMem.mod TicketLock.gvs)
+         (` b : bool <- OMod.call "compare" (x, SCMem.val_nat mytk);;
+          (if b then Ret () else tau;; TicketLock.lock_loop (SCMem.val_nat mytk)));;;
+         OMod.close_itree TicketLock.omod (SCMem.mod TicketLock.gvs) (trigger Yield)).
+  Proof.
+    iIntros "[#MYTN [MYTK MYNU]]". 
+    iopen 0 "I" "K". do 7 iDestruct "I" as "[% I]". iDestruct "I" as "[TKS [MEM [ST CASES]]]".
+    iPoseProof (mytk_find_some with "[MYTK TKS]") as "%FIND". iFrame.
+    iDestruct "CASES" as "[[%CT I] | [%CF [I | [I | I]]]]".
+    { iPoseProof (locked_myturn with "MYTN I") as "%FF". eauto. inv FF. }
+    { iPoseProof (unlocking_myturn with "MYTN I") as "%FF". eauto. inv FF. }
+    { iPoseProof (unlocked0_contra with "I") as "%FF". eauto. inv FF. }
+    iPoseProof (unlocked1_myturn with "MYTN I") as "%EQ". eauto. subst now.
+
+    unfold Mod.wrap_fun, SCMem.load_fun. rred.
+    iDestruct "MEM" as "[MEM0 [MEM1 [MEM2 MEM3]]]". iDestruct "ST" as "[ST0 ST1]".
+    iApply stsim_getR. iSplit. eauto. rred.
+    iApply stsim_tauR. rred.
+    iPoseProof (memory_ra_load with "MEM0 MEM1") as "%LOAD". des. rewrite LOAD. rred.
+    iApply stsim_tauR. rred.
+    rewrite close_itree_call. rred.
+
+    iMod ("K" with "[TKS MEM0 MEM1 MEM2 MEM3 ST0 ST1 I]") as "_".
+    { iExists mem, own, l, tks, mytk, next, myt. iFrame. iRight. iSplit; auto. }
+    clear pt mem own l tks next myt FIND CF LOAD LOAD0.
+    assert (exists tx0, tx = S tx0).
+    { inv TX; eauto. }
+    des. subst tx.
+    iApply lock_myturn_yieldR. iSplitL. iFrame. auto.
+    iIntros "[MYTK [MYNUM _]]". rred.
+
+    iopen 0 "I" "K". do 7 iDestruct "I" as "[% I]". iDestruct "I" as "[TKS [MEM [ST CASES]]]".
+    iPoseProof (mytk_find_some with "[MYTK TKS]") as "%FIND". iFrame.
+    iDestruct "CASES" as "[[%CT I] | [%CF [I | [I | I]]]]".
+    { iPoseProof (locked_myturn with "MYTN I") as "%FF". eauto. inv FF. }
+    { iPoseProof (unlocking_myturn with "MYTN I") as "%FF". eauto. inv FF. }
+    { iPoseProof (unlocked0_contra with "I") as "%FF". eauto. inv FF. }
+    iPoseProof (unlocked1_myturn with "MYTN I") as "%EQ". eauto. subst now.
+
+    unfold Mod.wrap_fun, SCMem.compare_fun. rred.
+    iDestruct "MEM" as "[MEM0 [MEM1 [MEM2 MEM3]]]". iDestruct "ST" as "[ST0 ST1]".
+    iApply stsim_getR. iSplit. eauto. rred.
+    iApply stsim_tauR. rred. iApply stsim_tauR. rred.
+    destruct (Nat.eq_dec mytk mytk).
+    2:{ exfalso. auto. }
+    clear e. subst. rred.
+
+    iApply stsim_yieldL. lred.
+    iApply stsim_getL. iSplit. auto. lred.
+    iApply stsim_getL. iSplit. auto.
+    iApply (stsim_putL with "ST1"). iIntros "ST1".
+
+    remember (NatMap.remove tid tks) as tks'.
+    rewrite <- key_set_pull_rm_eq. rewrite <- Heqtks'.
+    iAssert (ticket_lock_inv_state mem true tks')%I with "[ST0 ST1]" as "ST". iFrame.
+    iAssert (ticket_lock_inv_mem mem mytk next myt)%I with "[MEM0 MEM1 MEM2 MEM3]" as "MEM". iFrame.
+    iDestruct "TKS" as "[TKS0 [TKS1 [TKS2 TKS3]]]".
+    do 2 iDestruct "I" as "[% I]". iDestruct "I" as "[I0 [% [%I2 [I3 [I4 I5]]]]]".
+    do 3 iDestruct "I5" as "[% I5]". iDestruct "I5" as "[I5 [I6 [I7 [I8 [I9 I10]]]]]".
+    hexploit (tkqueue_inv_hd I2 _ FIND). i. des.
+    subst l. inversion H0; clear H0. subst yourt waits.
+
+    iPoseProof (NatMapRA_remove with "TKS0 MYTK") as ">TKS0". rewrite <- Heqtks'.
+    iPoseProof (natmap_prop_remove_find with "TKS2") as "[MYTH TKS2]". eauto. rewrite <- Heqtks'.
+    iCombine "I10 MYNUM" as "MYNUM". rewrite maps_to_res_add.
+    iPoseProof (OwnM_Upd with "MYNUM") as "> MYNUM".
+    { eapply maps_to_updatable. apply Auth.auth_update.
+      instantiate (1:=Excl.just 0). instantiate (1:=Excl.just 0).
+      ii. des. ur in FRAME. des_ifs. split; ur; ss.
+    }
+    iPoseProof (OwnMs_fold with "[TKS3 MYNUM]") as "TKS3".
+    2:{ iSplitL "TKS3". iFrame. iFrame. }
+    { instantiate (1:= fun id => ~ NatMap.In id tks'). i. ss. subst tks'.
+      destruct (tid_dec j tid); auto. left. ii. apply IN.
+      rewrite NatMapP.F.remove_neq_in_iff; auto.
+    }
+
+    iClear "I6 I9". iPoseProof (ObligationRA.pending_shot with "I7") as ">I7".
+    iPoseProof (ObligationRA.duty_done with "I8 I7") as ">DUTY".
+    iPoseProof (black_updatable with "I5") as ">I5".
+    { instantiate (1:=(mytk, Tkst.c k)). econs 2. ss. split; ss. lia. }
+    hexploit (tkqueue_dequeue I2).
+    { reflexivity. }
+    i. rename I2 into I2Old, H into I2. unfold TicketLockW.tk in I2. rewrite <- Heqtks' in I2.
+    iPoseProof (natmap_prop_remove with "I3") as "I3". rewrite <- Heqtks'.
+
+    iPoseProof (natmap_prop_sum_impl with "I3") as "I3".
+    { instantiate (1:= fun th tk =>
+                         ((FairRA.white th (Ord.from_nat (tk - (S mytk))))
+                            ∗ (FairRA.white th Ord.one))%I).
+      i. ss. iIntros "WHI". erewrite FairRA.white_eq.
+      2:{ instantiate (1:= (OrderedCM.add (Ord.from_nat (a - (S mytk))) (Ord.one))).
+          rewrite <- Ord.from_nat_1. ss. rewrite <- Hessenberg.add_from_nat. rr. ss.
+          hexploit (tkqueue_val_range_l I2 _ IN). i. split.
+          { apply OrdArith.le_from_nat. lia. }
+          { apply OrdArith.le_from_nat. lia. }
+      }
+      iPoseProof (FairRA.white_split with "WHI") as "[WHI1 WHI2]". iFrame.
+    }
+    iPoseProof (natmap_prop_sepconj_sum with "I3") as "[I3 TAX]".
+
+    iApply (stsim_fairL with "[TAX]").
+    { i. ss. instantiate (1:= (NatSet.elements (key_set tks'))). des_ifs. 
+      eapply NatSetIn_In. auto.
+    }
+    { instantiate (1:=[tid]). i; ss. des; clarify. des_ifs. }
+    { unfold natmap_prop_sum. unfold NatSet.elements. unfold nm_proj1.
+      unfold key_set. rewrite <- list_map_elements_nm_map. unfold unit1. rewrite List.map_map.
+      iPoseProof (list_prop_sum_map with "TAX") as "TAX".
+      2: iFrame.
+      ss. i. destruct a; ss.
+    }
+    instantiate (1:= Ord.omega). iIntros "[MYW _]".
+    iPoseProof (FairRA.whites_fold with "[TKS1 MYW]") as "TKS1".
+    2:{ iSplitL "TKS1". iFrame. iFrame. }
+    { instantiate (1:= fun id => ~ NatMap.In id tks'). ss. i. destruct (tid_dec j tid); auto.
+      left. ii. apply IN. subst tks'. rewrite NatMapP.F.remove_neq_in_iff; auto.
+    }
+
+    iMod ("K" with "[I0 I4 ST MEM TKS0 TKS2 TKS3 I5 I3 TKS1]") as "_".
+    { iExists mem, true, tl, tks', mytk, next, myt.
+      remember 
+    ((⌜true = true⌝ ** ticket_lock_inv_locked tl tks' mytk next myt)
+    ∨ (⌜true = false⌝ **
+       ticket_lock_inv_unlocking tl tks' mytk next myt
+       ∨ ticket_lock_inv_unlocked0 tl tks' mytk next myt
+       ∨ ticket_lock_inv_unlocked1 tl tks' mytk next myt))%I as temp.
+      iFrame. subst temp. iLeft. iSplit. auto.
+      iFrame. iSplit. auto. iExists k. iFrame.
+    }
+    iApply (stsim_sync with "[DUTY]"). msubtac. iFrame.
+    iIntros "DUTY _". rred.
+    iApply stsim_tauR. iApply stsim_ret. iModIntro. iFrame. auto.
+
+  Qed.
+
+  Lemma lock_myturn1
+        (g0 g1 : ∀ R_src R_tgt : Type,
+            (R_src → R_tgt → iProp)
+            → bool
+            → bool
+            → itree ((eventE +' cE) +' sE (Mod.state AbsLock.mod)) R_src
+            → itree ((eventE +' cE) +' sE (OMod.closed_state TicketLock.omod (SCMem.mod TicketLock.gvs))) R_tgt → iProp)
+        (ps pt: bool)
+        (tid : nat)
+        (mytk : TicketLockW.tk)
+        (mem : SCMem.t)
+        (own : bool)
+        (l : list nat)
+        (tks : NatMap.t nat)
+        (next myt : nat)
+    :
+  (OwnM (Auth.white (NatMapRA.singleton tid mytk: NatMapRA.t nat)) **
+   (maps_to tid (Auth.white (Excl.just 2: Excl.t nat)) **
+    (ticket_lock_inv_tks tks **
+     (ticket_lock_inv_mem mem mytk next myt **
+      (ticket_lock_inv_state mem own tks **
+       ((⌜own = true⌝ ** ticket_lock_inv_locked l tks mytk next myt)
+        ∨ (⌜own = false⌝ **
+           ticket_lock_inv_unlocking l tks mytk next myt
+           ∨ ticket_lock_inv_unlocked0 l tks mytk next myt
+             ∨ ticket_lock_inv_unlocked1 l tks mytk next myt) **
+        (ticket_lock_inv -*
+         MUpd (nth_default True%I I)
+           (fairI (ident_tgt:=OMod.closed_ident TicketLock.omod (SCMem.mod TicketLock.gvs))) []
+           [0] True)))))))
+  ⊢ (stsim I tid [] g0 g1
+      (λ r_src r_tgt : (), (own_thread tid ** ObligationRA.duty (inl tid) []) ** ⌜r_src = r_tgt⌝)
+      ps pt
+      (trigger Yield;;;
+       ` x : () + () <-
+       (` x_0 : bool * NatMap.t () <- trigger (Get (bool * NatMap.t ()));;
+        (let (own0, _) := x_0 in if Bool.eqb own0 true then Ret (inl ()) else Ret (inr ())));;
+       match x with
+       | inl l0 =>
+           tau;; ITree.iter
+                   (λ _ : (),
+                      trigger Yield;;;
+                      ` x_0 : bool * NatMap.t () <- trigger (Get (bool * NatMap.t ()));;
+                      (let (own0, _) := x_0 in
+                       if Bool.eqb own0 true then Ret (inl ()) else Ret (inr ()))) l0
+       | inr r0 => Ret r0
+       end;;;
+       ` x_0 : bool * NatMap.t () <- trigger (Get (bool * NatMap.t ()));;
+       (let (_, ts0) := x_0 in
+        trigger (Put (true, NatMap.remove (elt:=()) tid ts0));;;
+        trigger
+          (Fair
+             (λ i : nat,
+                if tid_dec i tid
+                then Flag.success
+                else
+                 if NatMapP.F.In_dec (NatMap.remove (elt:=()) tid ts0) i
+                 then Flag.fail
+                 else Flag.emp));;; trigger Yield;;; Ret ()))
+      (trigger Yield;;;
+       ` x : SCMem.val <-
+       (` rv : Any.t <-
+        OMod.embed_itree TicketLock.omod (SCMem.mod TicketLock.gvs)
+          (Mod.wrap_fun SCMem.load_fun (Any.upcast TicketLock.now_serving));;
+        (tau;; unwrap (Any.downcast rv)));;
+       OMod.close_itree TicketLock.omod (SCMem.mod TicketLock.gvs)
+         (` b : bool <- OMod.call "compare" (x, SCMem.val_nat mytk);;
+          (if b then Ret () else tau;; TicketLock.lock_loop (SCMem.val_nat mytk)));;;
+         OMod.close_itree TicketLock.omod (SCMem.mod TicketLock.gvs) (trigger Yield))).
+  Proof.
+    iIntros "[MYTK [MYN [TKS [MEM [ST [CASES K]]]]]]".
+    iAssert (⌜NatMap.find tid tks = Some mytk⌝)%I as "%FIND".
+    { iDestruct "TKS" as "[TKS0 _]". iApply (NatMapRA_find_some with "TKS0 MYTK"). }
+    iDestruct "CASES" as "[[%CT I] | [%CF [I | [I | I]]]]".
+    { iPoseProof (locked_contra with "I") as "%F". eauto. inv F. }
+    { iPoseProof (unlocking_contra with "I") as "%F". eauto. inv F. }
+    { iPoseProof (unlocked0_contra with "I") as "%F". eauto. inv F. }
+    iPoseProof (unlocked1_mono with "I") as "[%TKQ #MYMW]".
+    iDestruct "MYMW" as "[% [% [MYMW _]]]".
+    iMod ("K" with "[TKS MEM ST I]") as "_".
+    { iExists mem, own, l, tks, mytk, next, myt. iFrame. iRight. iSplit; auto. }
+    iApply lock_myturn_yieldR. iSplitL. iFrame. auto.
+    iIntros "[MYTK [MYN _]]". rred.
+    iApply lock_myturn0. 2: iFrame; auto. lia.
+  Qed.
+
+  Lemma lock_myturn2
+        (g0 g1 : ∀ R_src R_tgt : Type,
+            (R_src → R_tgt → iProp)
+            → bool
+            → bool
+            → itree ((eventE +' cE) +' sE (Mod.state AbsLock.mod)) R_src
+            → itree ((eventE +' cE) +' sE (OMod.closed_state TicketLock.omod (SCMem.mod TicketLock.gvs))) R_tgt → iProp)
+        (ps pt: bool)
+        (tid : nat)
+        (mytk : TicketLockW.tk)
+        (mem : SCMem.t)
+        (own : bool)
+        (l : list nat)
+        (tks : NatMap.t nat)
+        (next myt : nat)
+        now_old
+        (NEQ: mytk <> now_old)
+    :
+  (OwnM (Auth.white (NatMapRA.singleton tid mytk: NatMapRA.t nat)) **
+   (maps_to tid (Auth.white (Excl.just 2: Excl.t nat)) **
+    (ticket_lock_inv_tks tks **
+     (ticket_lock_inv_mem mem mytk next myt **
+      (ticket_lock_inv_state mem own tks **
+       ((⌜own = true⌝ ** ticket_lock_inv_locked l tks mytk next myt)
+        ∨ (⌜own = false⌝ **
+           ticket_lock_inv_unlocking l tks mytk next myt
+           ∨ ticket_lock_inv_unlocked0 l tks mytk next myt
+             ∨ ticket_lock_inv_unlocked1 l tks mytk next myt) **
+        (ticket_lock_inv -*
+         MUpd (nth_default True%I I)
+           (fairI (ident_tgt:=OMod.closed_ident TicketLock.omod (SCMem.mod TicketLock.gvs))) []
+           [0] True)))))))
+  ⊢ (stsim I tid [] g0 g1
+    (λ r_src r_tgt : (), (own_thread tid ** ObligationRA.duty (inl tid) []) ** ⌜r_src = r_tgt⌝)
+    ps pt
+    (trigger Yield;;;
+     ` x : () + () <-
+     (` x_0 : bool * NatMap.t () <- trigger (Get (bool * NatMap.t ()));;
+      (let (own0, _) := x_0 in if Bool.eqb own0 true then Ret (inl ()) else Ret (inr ())));;
+     match x with
+     | inl l0 =>
+         tau;; ITree.iter
+                 (λ _ : (),
+                    trigger Yield;;;
+                    ` x_0 : bool * NatMap.t () <- trigger (Get (bool * NatMap.t ()));;
+                    (let (own0, _) := x_0 in
+                     if Bool.eqb own0 true then Ret (inl ()) else Ret (inr ()))) l0
+     | inr r0 => Ret r0
+     end;;;
+     ` x_0 : bool * NatMap.t () <- trigger (Get (bool * NatMap.t ()));;
+     (let (_, ts0) := x_0 in
+      trigger (Put (true, NatMap.remove (elt:=()) tid ts0));;;
+      trigger
+        (Fair
+           (λ i : nat,
+              if tid_dec i tid
+              then Flag.success
+              else
+               if NatMapP.F.In_dec (NatMap.remove (elt:=()) tid ts0) i
+               then Flag.fail
+               else Flag.emp));;; trigger Yield;;; Ret ()))
+    (` r : Any.t <-
+     OMod.embed_itree TicketLock.omod (SCMem.mod TicketLock.gvs)
+       (Mod.wrap_fun SCMem.compare_fun (Any.upcast (SCMem.val_nat now_old, SCMem.val_nat mytk)));;
+     ` x : bool <- (tau;; unwrap (Any.downcast r));;
+     OMod.close_itree TicketLock.omod (SCMem.mod TicketLock.gvs)
+       (if x then Ret () else tau;; TicketLock.lock_loop (SCMem.val_nat mytk));;;
+       OMod.close_itree TicketLock.omod (SCMem.mod TicketLock.gvs) (trigger Yield))).
+  Proof.
+    iIntros "[MYTK [MYN [TKS [MEM [ST [CASES K]]]]]]".
+    unfold Mod.wrap_fun, SCMem.compare_fun. rred.
+    iDestruct "MEM" as "[MEM0 [MEM1 [MEM2 MEM3]]]". iDestruct "ST" as "[ST0 ST1]".
+    iApply stsim_getR. iSplit. eauto. rred.
+    iApply stsim_tauR. rred. iApply stsim_tauR. rred.
+    destruct (Nat.eq_dec now_old mytk).
+    { exfalso. clarify. }
+    rred. iApply stsim_tauR.
+    rewrite TicketLock.lock_loop_red. rred. rewrite close_itree_call. rred.
+    iApply lock_myturn1.
+    iSplitL "MYTK". iFrame. iSplitL "MYN". iFrame. iSplitL "TKS". iFrame.
+    iSplitL "MEM0 MEM1 MEM2 MEM3". iFrame. iSplitL "ST0 ST1". iFrame. iSplitL "CASES". iFrame.
+    iFrame.
+  Qed.
+
+  Let src_code_coind tid: itree ((eventE +' cE) +' sE (Mod.state AbsLock.mod)) () :=
+          ((` lr : () + () <-
+            (trigger Yield;;;
+             ` x_0 : bool * NatMap.t () <- trigger (Get (bool * NatMap.t ()));;
+             (let (own0, _) := x_0 in if Bool.eqb own0 true then Ret (inl ()) else Ret (inr ())));;
+            match lr with
+            | inl l0 =>
+                tau;; ITree.iter
+                        (λ _ : (),
+                           trigger Yield;;;
+                           ` x_0 : bool * NatMap.t () <- trigger (Get (bool * NatMap.t ()));;
+                           (let (own0, _) := x_0 in
+                            if Bool.eqb own0 true then Ret (inl ()) else Ret (inr ()))) l0
+            | inr r0 => Ret r0
+            end);;;
+           ` x_0 : bool * NatMap.t () <- trigger (Get (bool * NatMap.t ()));;
+           (let (_, ts0) := x_0 in
+            trigger (Put (true, NatMap.remove (elt:=()) tid ts0));;;
+            trigger
+              (Fair
+                 (λ i : nat,
+                    if tid_dec i tid
+                    then Flag.success
+                    else
+                     if NatMapP.F.In_dec (NatMap.remove (elt:=()) tid ts0) i
+                     then Flag.fail
+                     else Flag.emp));;; trigger Yield;;; Ret ())).
+
+  Let tgt_code_coind a :=
+          (trigger Yield;;;
+           ` x : SCMem.val <-
+           (` rv : Any.t <-
+            OMod.embed_itree TicketLock.omod (SCMem.mod TicketLock.gvs)
+              (` arg : SCMem.val <- unwrap (Any.downcast (Any.upcast TicketLock.now_serving));;
+               ` ret : SCMem.val <-
+               (` m : SCMem.t <- trigger (Get SCMem.t);;
+                ` v : SCMem.val <- unwrap (SCMem.load m arg);; Ret v);; 
+               Ret (Any.upcast ret));; (tau;; unwrap (Any.downcast rv)));;
+           OMod.close_itree TicketLock.omod (SCMem.mod TicketLock.gvs)
+             (` b : bool <- OMod.call "compare" (x, SCMem.val_nat a);;
+              (if b then Ret () else tau;; TicketLock.lock_loop (SCMem.val_nat a)));;;
+           OMod.close_itree TicketLock.omod (SCMem.mod TicketLock.gvs) (trigger Yield)).
+
+  Lemma lock_yourturn_coind
+        (g0 g1 : ∀ R_src R_tgt : Type,
+            (R_src → R_tgt → iProp)
+            → bool
+            → bool
+            → itree ((eventE +' cE) +' sE (Mod.state AbsLock.mod)) R_src
+            → itree ((eventE +' cE) +' sE (OMod.closed_state TicketLock.omod (SCMem.mod TicketLock.gvs))) R_tgt → iProp)
+        (ps pt: bool)
+        (tid : nat)
+        (mytk : TicketLockW.tk)
+        (mem : SCMem.t)
+        (l : list nat)
+        (tks : NatMap.t nat)
+        (now next myt : nat)
+        now_old
+        (NEQ: mytk <> now_old)
+    :
+  (□ (∀ a : TicketLockW.tk,
+        (OwnM (Auth.white (NatMapRA.singleton tid a: NatMapRA.t nat)) ** maps_to tid (Auth.white (Excl.just 2: Excl.t nat))) -*
+        g1 ()%type ()%type
+          (λ r_src r_tgt : (),
+              (own_thread tid ** ObligationRA.duty (inl tid) []) ** ⌜r_src = r_tgt⌝) false false
+          (src_code_coind tid)
+          (tgt_code_coind a)
+     ) **
+   (maps_to tid (Auth.white (Excl.just 2: Excl.t nat)) **
+    (OwnM (Auth.white (NatMapRA.singleton tid mytk: NatMapRA.t nat)) **
+     (ticket_lock_inv_tks tks **
+      (ticket_lock_inv_mem mem now next myt **
+       (ticket_lock_inv_state mem true tks **
+        (ticket_lock_inv_locked l tks now next myt **
+         (ticket_lock_inv -*
+          MUpd (nth_default True%I I)
+            (fairI (ident_tgt:=OMod.closed_ident TicketLock.omod (SCMem.mod TicketLock.gvs))) []
+            [0] True)))))))
+  )
+  ⊢ (stsim I tid [] g0 g1
+      (λ r_src r_tgt : (), (own_thread tid ** ObligationRA.duty (inl tid) []) ** ⌜r_src = r_tgt⌝)
+      ps pt
+      (trigger Yield;;;
+       ` x : () + () <-
+       (` x_0 : bool * NatMap.t () <- trigger (Get (bool * NatMap.t ()));;
+        (let (own0, _) := x_0 in if Bool.eqb own0 true then Ret (inl ()) else Ret (inr ())));;
+       match x with
+       | inl l0 =>
+           tau;; ITree.iter
+                   (λ _ : (),
+                      trigger Yield;;;
+                      ` x_0 : bool * NatMap.t () <- trigger (Get (bool * NatMap.t ()));;
+                      (let (own0, _) := x_0 in
+                       if Bool.eqb own0 true then Ret (inl ()) else Ret (inr ()))) l0
+       | inr r0 => Ret r0
+       end;;;
+       ` x_0 : bool * NatMap.t () <- trigger (Get (bool * NatMap.t ()));;
+       (let (_, ts0) := x_0 in
+        trigger (Put (true, NatMap.remove (elt:=()) tid ts0));;;
+        trigger
+          (Fair
+             (λ i : nat,
+                if tid_dec i tid
+                then Flag.success
+                else
+                 if NatMapP.F.In_dec (NatMap.remove (elt:=()) tid ts0) i
+                 then Flag.fail
+                 else Flag.emp));;; trigger Yield;;; Ret ()))
+      (` r : Any.t <-
+       OMod.embed_itree TicketLock.omod (SCMem.mod TicketLock.gvs)
+         (Mod.wrap_fun SCMem.compare_fun (Any.upcast (SCMem.val_nat now_old, SCMem.val_nat mytk)));;
+       ` x : bool <- (tau;; unwrap (Any.downcast r));;
+       OMod.close_itree TicketLock.omod (SCMem.mod TicketLock.gvs)
+         (if x then Ret () else tau;; TicketLock.lock_loop (SCMem.val_nat mytk));;;
+       OMod.close_itree TicketLock.omod (SCMem.mod TicketLock.gvs) (trigger Yield))).
+  Proof.
+    iIntros "[#CIH [MYTK [MYN [TKS [MEM [ST [I K]]]]]]]".
+    unfold Mod.wrap_fun, SCMem.compare_fun. rred.
+    iDestruct "MEM" as "[MEM0 [MEM1 [MEM2 MEM3]]]". iDestruct "ST" as "[ST0 ST1]".
+    iApply stsim_getR. iSplit. eauto. rred.
+    iApply stsim_tauR. rred. iApply stsim_tauR. rred.
+    destruct (Nat.eq_dec now_old mytk).
+    { exfalso. clarify. }
+    rred. iApply stsim_tauR.
+    rewrite TicketLock.lock_loop_red. rred. rewrite close_itree_call. rred.
+
+    iApply stsim_yieldL. lred.
+    iApply stsim_getL. iSplit. auto. lred.
+    iApply stsim_tauL.
+    iMod ("K" with "[TKS MEM0 MEM1 MEM2 MEM3 ST0 ST1 I]") as "_".
+    { do 7 iExists _.
+      iSplitL "TKS". iFrame. iSplitL "MEM0 MEM1 MEM2 MEM3". iFrame.
+      iSplitL "ST0 ST1". iFrame.
+      iLeft. iSplit. auto. iFrame.
+    }
+    iApply stsim_progress. iApply stsim_base. msubtac.
+    rewrite unfold_iter_eq. iApply "CIH". iFrame.
+  Qed.
+
+  Lemma yourturn_range
+        tid tks mytk now next own l myt
+        (FIND : NatMap.find tid tks = Some mytk)
+        (NEQ : mytk ≠ now)
+    :
+    ((⌜own = true⌝ ∗ ticket_lock_inv_locked l tks now next myt)
+     ∨ (⌜own = false⌝ ∗
+                    (ticket_lock_inv_unlocking l tks now next myt
+                     ∨ ticket_lock_inv_unlocked0 l tks now next myt
+                     ∨ ticket_lock_inv_unlocked1 l tks now next myt)))
+      ⊢
+      (⌜now < mytk⌝).
+  Proof.
+    iIntros "[[%CT I] | [%CF [I | [I | I]]]]".
+    { iDestruct "I" as "[_ [%I1 _]]".
+      hexploit (tkqueue_val_range_l I1 _ FIND). i. iPureIntro. lia. }
+    { iDestruct "I" as "[_ [%I1 _]]".
+      hexploit (tkqueue_val_range_l I1 _ FIND). i. iPureIntro. lia. }
+    { iPoseProof (unlocked0_contra with "I") as "%FF". eauto. inv FF. }
+    { iPoseProof (unlocked1_mono with "I") as "[%I1 _]".
+      hexploit (tkqueue_val_range_l I1 _ FIND). i. iPureIntro. lia. }
+  Qed.
+
+  Let src_code_ind tid: itree ((eventE +' cE) +' sE (Mod.state AbsLock.mod)) () :=
+                         (trigger Yield;;;
+                          ` x : () + () <-
+                          (` x_0 : bool * NatMap.t () <- trigger (Get (bool * NatMap.t ()));;
+                           (let (own0, _) := x_0 in
+                            if Bool.eqb own0 true then Ret (inl ()) else Ret (inr ())));;
+                          match x with
+                          | inl l0 =>
+                              tau;; ITree.iter
+                                      (λ _ : (),
+                                         trigger Yield;;;
+                                         ` x_0 : bool * NatMap.t () <-
+                                         trigger (Get (bool * NatMap.t ()));;
+                                         (let (own0, _) := x_0 in
+                                          if Bool.eqb own0 true
+                                          then Ret (inl ())
+                                          else Ret (inr ()))) l0
+                          | inr r0 => Ret r0
+                          end;;;
+                          ` x_0 : bool * NatMap.t () <- trigger (Get (bool * NatMap.t ()));;
+                          (let (_, ts0) := x_0 in
+                           trigger (Put (true, NatMap.remove (elt:=()) tid ts0));;;
+                           trigger
+                             (Fair
+                                (λ i : nat,
+                                   if tid_dec i tid
+                                   then Flag.success
+                                   else
+                                    if NatMapP.F.In_dec (NatMap.remove (elt:=()) tid ts0) i
+                                    then Flag.fail
+                                    else Flag.emp));;; trigger Yield;;; Ret ())).
+
+  Let tgt_code_ind mytk now_old :=
+                         (` r : Any.t <-
+                          OMod.embed_itree TicketLock.omod (SCMem.mod TicketLock.gvs)
+                            (Mod.wrap_fun SCMem.compare_fun
+                               (Any.upcast (SCMem.val_nat now_old, SCMem.val_nat mytk)));;
+                          ` x : bool <- (tau;; unwrap (Any.downcast r));;
+                          OMod.close_itree TicketLock.omod (SCMem.mod TicketLock.gvs)
+                            (if x
+                             then Ret ()
+                             else tau;; TicketLock.lock_loop (SCMem.val_nat mytk));;;
+                          OMod.close_itree TicketLock.omod (SCMem.mod TicketLock.gvs)
+                            (trigger Yield)).
+
+  Lemma lock_yourturn_ind0
+        (g0 g1 : ∀ R_src R_tgt : Type,
+            (R_src → R_tgt → iProp)
+            → bool
+            → bool
+            → itree ((eventE +' cE) +' sE (Mod.state AbsLock.mod)) R_src
+            → itree ((eventE +' cE) +' sE (OMod.closed_state TicketLock.omod (SCMem.mod TicketLock.gvs))) R_tgt → iProp)
+        (tid : nat)
+        (mytk : TicketLockW.tk)
+  (now : nat)
+  (LT : now < mytk)
+  (IH : ∀ y : nat,
+         y < mytk - now
+         → ∀ now_old : nat,
+             mytk ≠ now_old
+             → ∀ (mem : SCMem.t) (own : bool) (l : list nat) (tks : NatMap.t nat)
+                 (now next myt : nat),
+                 now < mytk
+                 → y = mytk - now
+                   → (□ ((∀ a : TicketLockW.tk,
+                            (OwnM (Auth.white (NatMapRA.singleton tid a: NatMapRA.t nat)) **
+                             maps_to tid (Auth.white (Excl.just 2: Excl.t nat))) -*
+                            g1 ()%type ()%type
+                              (λ r_src r_tgt : (),
+                                 (own_thread tid ** ObligationRA.duty (inl tid) []) **
+                                 ⌜r_src = r_tgt⌝) false false
+                              (src_code_coind tid)
+                              (tgt_code_coind a)
+                         ) ∧ monoWhite tk_mono Nat.le_preorder now) **
+                      (maps_to tid (Auth.white (Excl.just 2: Excl.t nat)) **
+                       (OwnM (Auth.white (NatMapRA.singleton tid mytk: NatMapRA.t nat)) **
+                        (ticket_lock_inv_tks tks **
+                         (ticket_lock_inv_state mem own tks **
+                          ((⌜own = true⌝ ** ticket_lock_inv_locked l tks now next myt)
+                           ∨ (⌜own = false⌝ **
+                              ticket_lock_inv_unlocking l tks now next myt
+                              ∨ ticket_lock_inv_unlocked0 l tks now next myt
+                                ∨ ticket_lock_inv_unlocked1 l tks now next myt) **
+                           ((ticket_lock_inv -*
+                             MUpd (nth_default True%I I)
+                               (fairI
+                                  (ident_tgt:=OMod.closed_ident TicketLock.omod
+                                                (SCMem.mod TicketLock.gvs))) [] [0] True) **
+                            ticket_lock_inv_mem mem now next myt)))))))
+                     ⊢ stsim I tid [] g0 g1
+                         (λ r_src r_tgt : (),
+                            (own_thread tid ** ObligationRA.duty (inl tid) []) ** ⌜r_src = r_tgt⌝)
+                         false true
+                         (src_code_ind tid)
+                         (tgt_code_ind mytk now_old)
+  )
+  (now_old : nat)
+  (NEQ : mytk ≠ now_old)
+  (mem : SCMem.t)
+  (l : list nat)
+  (tks : NatMap.t nat)
+  (next myt : nat)
+    :
+  (□ ((∀ a : TicketLockW.tk,
+        (OwnM (Auth.white (NatMapRA.singleton tid a: NatMapRA.t nat)) ** maps_to tid (Auth.white (Excl.just 2: Excl.t nat))) -*
+        g1 ()%type ()%type
+          (λ r_src r_tgt : (),
+             (own_thread tid ** ObligationRA.duty (inl tid) []) ** ⌜r_src = r_tgt⌝) false false
+          (src_code_coind tid)
+          (tgt_code_coind a))
+          ∧
+  (monoWhite tk_mono Nat.le_preorder now)
+     ) **
+   (maps_to tid (Auth.white (Excl.just 2: Excl.t nat)) **
+    (OwnM (Auth.white (NatMapRA.singleton tid mytk: NatMapRA.t nat)) **
+     (ticket_lock_inv_tks tks **
+      (ticket_lock_inv_mem mem now next myt **
+       (ticket_lock_inv_state mem false tks **
+        (ticket_lock_inv_unlocking l tks now next myt **
+         (ticket_lock_inv -*
+          MUpd (nth_default True%I I)
+            (fairI (ident_tgt:=OMod.closed_ident TicketLock.omod (SCMem.mod TicketLock.gvs))) []
+            [0] True)))))))
+  )
+  ⊢ (stsim I tid [] g0 g1
+      (λ r_src r_tgt : (), (own_thread tid ** ObligationRA.duty (inl tid) []) ** ⌜r_src = r_tgt⌝)
+      false true
+      (trigger Yield;;;
+       ` x : () + () <-
+       (` x_0 : bool * NatMap.t () <- trigger (Get (bool * NatMap.t ()));;
+        (let (own0, _) := x_0 in if Bool.eqb own0 true then Ret (inl ()) else Ret (inr ())));;
+       match x with
+       | inl l0 =>
+           tau;; ITree.iter
+                   (λ _ : (),
+                      trigger Yield;;;
+                      ` x_0 : bool * NatMap.t () <- trigger (Get (bool * NatMap.t ()));;
+                      (let (own0, _) := x_0 in
+                       if Bool.eqb own0 true then Ret (inl ()) else Ret (inr ()))) l0
+       | inr r0 => Ret r0
+       end;;;
+       ` x_0 : bool * NatMap.t () <- trigger (Get (bool * NatMap.t ()));;
+       (let (_, ts0) := x_0 in
+        trigger (Put (true, NatMap.remove (elt:=()) tid ts0));;;
+        trigger
+          (Fair
+             (λ i : nat,
+                if tid_dec i tid
+                then Flag.success
+                else
+                 if NatMapP.F.In_dec (NatMap.remove (elt:=()) tid ts0) i
+                 then Flag.fail
+                 else Flag.emp));;; trigger Yield;;; Ret ()))
+      (` r : Any.t <-
+       OMod.embed_itree TicketLock.omod (SCMem.mod TicketLock.gvs)
+         (Mod.wrap_fun SCMem.compare_fun (Any.upcast (SCMem.val_nat now_old, SCMem.val_nat mytk)));;
+       ` x : bool <- (tau;; unwrap (Any.downcast r));;
+       OMod.close_itree TicketLock.omod (SCMem.mod TicketLock.gvs)
+         (if x then Ret () else tau;; TicketLock.lock_loop (SCMem.val_nat mytk));;;
+       OMod.close_itree TicketLock.omod (SCMem.mod TicketLock.gvs) (trigger Yield))).
+  Proof.
+    iIntros "[#[CIH MONOTK] [MYN [MYTK [TKS [MEM [ST [I K]]]]]]]".
+    iPoseProof (mytk_find_some with "[MYTK TKS]") as "%FIND". iFrame.
+    iPoseProof (unlocking_mono with "I") as "[%TKQ #[% [% [MONOW OBLB]]]]".
+    clear FIND TKQ.
+    iStopProof. move o before IH. revert_until o. pattern o. revert o.
+    apply (well_founded_induction Ord.lt_well_founded).
+    intros o IHo. intros.
+    iIntros "[#[CIH [MONOTK [MONOW BLK]]] [MYN [MYTK [TKS [MEM [ST [I K]]]]]]]".
+
+    unfold Mod.wrap_fun, SCMem.compare_fun. rred.
+    iDestruct "MEM" as "[MEM0 [MEM1 [MEM2 MEM3]]]". iDestruct "ST" as "[ST0 ST1]".
+    iApply stsim_getR. iSplit. eauto. rred.
+    iApply stsim_tauR. rred. iApply stsim_tauR. rred.
+    destruct (Nat.eq_dec now_old mytk).
+    { exfalso. clarify. }
+    rred. iApply stsim_tauR.
+    rewrite TicketLock.lock_loop_red. rred. rewrite close_itree_call. rred.
+    iAssert (ticket_lock_inv_mem mem now next myt)%I with "[MEM0 MEM1 MEM2 MEM3]" as "MEM". iFrame.
+    iAssert (ticket_lock_inv_state mem false tks)%I with "[ST0 ST1]" as "ST". iFrame.
+    iMod ("K" with "[TKS MEM ST I]") as "_".
+    { do 7 iExists _. iSplitL "TKS". iFrame. iSplitL "MEM". iFrame. iSplitL "ST". iFrame.
+      iRight. iSplit. auto. iLeft. iFrame.
+    }
+    clear mem l tks next myt now_old NEQ n.
+    rename now into now_past, LT into LTPAST, k into k_past, o into o_past.
+
+    iopen 0 "I" "K". do 7 iDestruct "I" as "[% I]". iDestruct "I" as "[TKS [MEM [ST CASES]]]".
+    destruct (Nat.eq_dec mytk now); subst.
+    { iClear "CIH".
+      iApply lock_myturn1.
+      iSplitL "MYTK". iFrame. iSplitL "MYN". iFrame. iSplitL "TKS". iFrame.
+      iSplitL "MEM". iFrame. iSplitL "ST". iFrame. iSplitL "CASES". iFrame.
+      iFrame.
+    }
+
+    rename n into NEQ.
+    iApply lock_yourturn_yieldR. eapply NEQ.
+    iSplitL "MYTK TKS MEM ST CASES K".
+    iSplitL "MYTK". iFrame. iSplitL "TKS". iFrame. iSplitL "MEM". iFrame.
+    iSplitL "ST". iFrame. iSplitL "CASES". iFrame. iFrame.
+    iIntros "[MYTK _]". rred.
+    clear mem own l tks now next myt NEQ.
+    iopen 0 "I" "K". do 7 iDestruct "I" as "[% I]". iDestruct "I" as "[TKS [MEM [ST CASES]]]".
+    destruct (Nat.eq_dec mytk now); subst.
+    { iClear "CIH".
+      iPoseProof (mytk_find_some with "[MYTK TKS]") as "%FIND". iFrame.
+      iDestruct "CASES" as "[[%CT I] | [%CF [I | [I | I]]]]".
+      { iPoseProof (locked_contra with "I") as "%F". eauto. inv F. }
+      { iPoseProof (unlocking_contra with "I") as "%F". eauto. inv F. }
+      { iPoseProof (unlocked0_contra with "I") as "%F". eauto. inv F. }
+      iPoseProof (unlocked1_mono with "I") as "[%TKQ #[% [% [MYTN _]]]]".
+      iMod ("K" with "[TKS MEM ST I]") as "_".
+      { do 7 iExists _. iSplitL "TKS". iFrame. iSplitL "MEM". iFrame. iSplitL "ST". iFrame.
+        iRight. iSplit. auto. iFrame.
+      }
+      iApply lock_myturn0. 2: iFrame; auto. lia.
+    }
+
+    rename n into NEQ. unfold Mod.wrap_fun, SCMem.load_fun. rred.
+    iDestruct "MEM" as "[MEM0 [MEM1 [MEM2 MEM3]]]". iDestruct "ST" as "[ST0 ST1]".
+    iApply stsim_getR. iSplit. eauto. rred.
+    iApply stsim_tauR. rred.
+    iPoseProof (memory_ra_load with "MEM0 MEM1") as "%LOAD". des. rewrite LOAD. rred.
+    iApply stsim_tauR. rred.
+    rewrite close_itree_call. rred.
+    iApply lock_yourturn_yieldR. eapply NEQ.
+    iSplitL "MYTK TKS MEM0 MEM1 MEM2 MEM3 ST0 ST1 CASES K".
+    iSplitL "MYTK". iFrame. iSplitL "TKS". iFrame. iSplitL "MEM0 MEM1 MEM2 MEM3". iFrame.
+    iSplitL "ST0 ST1". iFrame. iSplitL "CASES". iFrame. iFrame.
+    iIntros "[MYTK RIGHT]". rred.
+    rename now into now_old. clear mem own l tks next myt LOAD LOAD0.
+
+    iopen 0 "I" "K". do 7 iDestruct "I" as "[% I]". iDestruct "I" as "[TKS [MEM [ST CASES]]]".
+    destruct (Nat.eq_dec mytk now); subst.
+    { iClear "CIH". iApply lock_myturn2. auto.
+      iSplitL "MYTK". iFrame. iSplitL "MYN". iFrame. iSplitL "TKS". iFrame.
+      iSplitL "MEM". iFrame. iSplitL "ST". iFrame. iSplitL "CASES". iFrame.
+      iFrame.
+    }
+
+    iPoseProof (mytk_find_some with "[MYTK TKS]") as "%FIND". iFrame.
+    rename n into NEQ2. iPoseProof (yourturn_range with "CASES") as "%LT". eapply FIND. auto.
+    clear NEQ2. iDestruct "CASES" as "[[%CT I] | [%CF [I | [I | I]]]]".
+    { subst own. iApply lock_yourturn_coind. auto. iSplit. iApply "CIH".
+      iSplitL "MYN". iFrame. iSplitL "MYTK". iFrame. iSplitL "TKS". iFrame.
+      iSplitL "MEM". iFrame. iSplitL "ST". iFrame. iSplitL "I". iFrame. iFrame.
+    }
+
+    { iPoseProof (ticket_lock_inv_mem_mono with "MEM") as "#MONOTK2".
+      iDestruct "I" as "[I0 [%I1 [I2 [I3 I4]]]]".
+      do 2 iDestruct "I4" as "[% I4]". iDestruct "I4" as "[I4 [I5 [I6 I7]]]".
+      iPoseProof (black_white_compare with "MONOW I4") as "%LE".
+      inv LE.
+      { remember (mytk - now) as ind. specialize (IH ind).
+        iApply IH.
+        { subst ind. lia. }
+        { auto. }
+        { eapply LT. }
+        { eapply Heqind. }
+        iSplit.
+        { iClear "MYN MYTK RIGHT TKS MEM ST I0 I2 I3 I4 I5 I6 I7 K".
+          iModIntro. iSplit. iApply "CIH". auto.
+        }
+        iSplitL "MYN". iFrame. iSplitL "MYTK". iFrame. iSplitL "TKS". iFrame.
+        iSplitL "ST". iFrame. iSplitR "K MEM". 2: iFrame.
+        iRight. iSplit. auto. iLeft. iFrame. iSplit. auto. iExists _, _. iFrame.
+      }
+      { inv ORD. hexploit H0. lia. i. clear H H0. subst k.
+        iClear "MONOTK2".
+        iPoseProof (ObligationRA.duty_correl_thread with "I7") as "#COR".
+        { ss. left; eauto. }
+        iPoseProof (ObligationRA.correl_thread_correlate with "COR RIGHT") as ">[DROP | FF]".
+        2:{ iPoseProof (ObligationRA.pending_not_shot with "I6 FF") as "%FF". inv FF. }
+        iPoseProof (ObligationRA.black_white_decr with "BLK DROP") as ">[%o_now [#OBLK2 %DROP]]".
+        iClear "BLK".
+        specialize (IHo o_now).
+        iApply IHo.
+        { rewrite Hessenberg.add_S_r in DROP. rewrite Hessenberg.add_O_r in DROP.
+          eapply Ord.lt_le_lt. 2: eapply DROP. apply Ord.S_lt.
+        }
+        { auto. }
+        iSplit.
+        { iClear "MYN MYTK TKS MEM ST I0 I2 I3 I4 I5 I6 I7 K".
+          iModIntro. iSplit. iApply "CIH". iSplit; auto.
+        }
+        iSplitL "MYN". iFrame. iSplitL "MYTK". iFrame. iSplitL "TKS". iFrame.
+        iSplitL "MEM". iFrame. iSplitL "ST". iFrame. iSplitR "K". 2: iFrame.
+        iFrame. iSplit. auto. iExists _, _. iFrame.
+      }
+    }
+    { iPoseProof (unlocked0_contra with "I") as "%FF". eauto. inv FF. }
+
+    { iPoseProof (ticket_lock_inv_mem_mono with "MEM") as "#MONOTK2".
+      do 2 iDestruct "I" as "[% I]". iDestruct "I" as "[I0 [I1 [%I2 [I3 [I4 I5]]]]]".
+      do 3 iDestruct "I5" as "[% I5]". iDestruct "I5" as "[I5 [I6 [I7 [I8 [I9 I10]]]]]".
+      iPoseProof (black_white_compare with "MONOW I5") as "%LE".
+      inv LE.
+      { remember (mytk - now) as ind. specialize (IH ind).
+        iApply IH.
+        { subst ind. lia. }
+        { auto. }
+        { eapply LT. }
+        { eapply Heqind. }
+        iSplit.
+        { iClear "MYN MYTK RIGHT TKS MEM ST I0 I1 I3 I4 I5 I6 I7 I8 I9 I10 K".
+          iModIntro. iSplit. iApply "CIH". auto.
+        }
+        iSplitL "MYN". iFrame. iSplitL "MYTK". iFrame. iSplitL "TKS". iFrame.
+        iSplitL "ST". iFrame. iSplitR "K MEM". 2: iFrame.
+        iRight. iSplit. auto. iRight. iRight. iFrame.
+        iExists yourt, waits. iSplit. auto. iSplit. auto. iFrame.
+        iExists k, o, u. iFrame.
+      }
+      { exfalso. inv ORD. lia. }
+    }
+  Qed.
+
+  Lemma lock_yourturn_ind1
+        (g0 g1 : ∀ R_src R_tgt : Type,
+            (R_src → R_tgt → iProp)
+            → bool
+            → bool
+            → itree ((eventE +' cE) +' sE (Mod.state AbsLock.mod)) R_src
+            → itree ((eventE +' cE) +' sE (OMod.closed_state TicketLock.omod (SCMem.mod TicketLock.gvs))) R_tgt → iProp)
+        (tid : nat)
+        (mytk : TicketLockW.tk)
+  (now : nat)
+  (LT : now < mytk)
+  (IH : ∀ y : nat,
+         y < mytk - now
+         → ∀ now_old : nat,
+             mytk ≠ now_old
+             → ∀ (mem : SCMem.t) (own : bool) (l : list nat) (tks : NatMap.t nat)
+                 (now next myt : nat),
+                 now < mytk
+                 → y = mytk - now
+                   → (□ ((∀ a : TicketLockW.tk,
+                            (OwnM (Auth.white (NatMapRA.singleton tid a: NatMapRA.t nat)) **
+                             maps_to tid (Auth.white (Excl.just 2: Excl.t nat))) -*
+                            g1 ()%type ()%type
+                              (λ r_src r_tgt : (),
+                                 (own_thread tid ** ObligationRA.duty (inl tid) []) **
+                                 ⌜r_src = r_tgt⌝) false false
+                              (src_code_coind tid)
+                              (tgt_code_coind a)
+                         ) ∧ monoWhite tk_mono Nat.le_preorder now) **
+                      (maps_to tid (Auth.white (Excl.just 2: Excl.t nat)) **
+                       (OwnM (Auth.white (NatMapRA.singleton tid mytk: NatMapRA.t nat)) **
+                        (ticket_lock_inv_tks tks **
+                         (ticket_lock_inv_state mem own tks **
+                          ((⌜own = true⌝ ** ticket_lock_inv_locked l tks now next myt)
+                           ∨ (⌜own = false⌝ **
+                              ticket_lock_inv_unlocking l tks now next myt
+                              ∨ ticket_lock_inv_unlocked0 l tks now next myt
+                                ∨ ticket_lock_inv_unlocked1 l tks now next myt) **
+                           ((ticket_lock_inv -*
+                             MUpd (nth_default True%I I)
+                               (fairI
+                                  (ident_tgt:=OMod.closed_ident TicketLock.omod
+                                                (SCMem.mod TicketLock.gvs))) [] [0] True) **
+                            ticket_lock_inv_mem mem now next myt)))))))
+                     ⊢ stsim I tid [] g0 g1
+                         (λ r_src r_tgt : (),
+                            (own_thread tid ** ObligationRA.duty (inl tid) []) ** ⌜r_src = r_tgt⌝)
+                         false true
+                         (src_code_ind tid)
+                         (tgt_code_ind mytk now_old)
+  )
+  (now_old : nat)
+  (NEQ : mytk ≠ now_old)
+  (mem : SCMem.t)
+  (l : list nat)
+  (tks : NatMap.t nat)
+  (next myt : nat)
+    :
+  (□ ((∀ a : TicketLockW.tk,
+        (OwnM (Auth.white (NatMapRA.singleton tid a: NatMapRA.t nat)) ** maps_to tid (Auth.white (Excl.just 2: Excl.t nat))) -*
+        g1 ()%type ()%type
+          (λ r_src r_tgt : (),
+             (own_thread tid ** ObligationRA.duty (inl tid) []) ** ⌜r_src = r_tgt⌝) false false
+          (src_code_coind tid)
+          (tgt_code_coind a))
+          ∧
+  (monoWhite tk_mono Nat.le_preorder now)
+     ) **
+   (maps_to tid (Auth.white (Excl.just 2: Excl.t nat)) **
+    (OwnM (Auth.white (NatMapRA.singleton tid mytk: NatMapRA.t nat)) **
+     (ticket_lock_inv_tks tks **
+      (ticket_lock_inv_mem mem now next myt **
+       (ticket_lock_inv_state mem false tks **
+        (ticket_lock_inv_unlocked1 l tks now next myt **
+         (ticket_lock_inv -*
+          MUpd (nth_default True%I I)
+            (fairI (ident_tgt:=OMod.closed_ident TicketLock.omod (SCMem.mod TicketLock.gvs))) []
+            [0] True)))))))
+  )
+  ⊢ (stsim I tid [] g0 g1
+      (λ r_src r_tgt : (), (own_thread tid ** ObligationRA.duty (inl tid) []) ** ⌜r_src = r_tgt⌝)
+      false true
+      (trigger Yield;;;
+       ` x : () + () <-
+       (` x_0 : bool * NatMap.t () <- trigger (Get (bool * NatMap.t ()));;
+        (let (own0, _) := x_0 in if Bool.eqb own0 true then Ret (inl ()) else Ret (inr ())));;
+       match x with
+       | inl l0 =>
+           tau;; ITree.iter
+                   (λ _ : (),
+                      trigger Yield;;;
+                      ` x_0 : bool * NatMap.t () <- trigger (Get (bool * NatMap.t ()));;
+                      (let (own0, _) := x_0 in
+                       if Bool.eqb own0 true then Ret (inl ()) else Ret (inr ()))) l0
+       | inr r0 => Ret r0
+       end;;;
+       ` x_0 : bool * NatMap.t () <- trigger (Get (bool * NatMap.t ()));;
+       (let (_, ts0) := x_0 in
+        trigger (Put (true, NatMap.remove (elt:=()) tid ts0));;;
+        trigger
+          (Fair
+             (λ i : nat,
+                if tid_dec i tid
+                then Flag.success
+                else
+                 if NatMapP.F.In_dec (NatMap.remove (elt:=()) tid ts0) i
+                 then Flag.fail
+                 else Flag.emp));;; trigger Yield;;; Ret ()))
+      (` r : Any.t <-
+       OMod.embed_itree TicketLock.omod (SCMem.mod TicketLock.gvs)
+         (Mod.wrap_fun SCMem.compare_fun (Any.upcast (SCMem.val_nat now_old, SCMem.val_nat mytk)));;
+       ` x : bool <- (tau;; unwrap (Any.downcast r));;
+       OMod.close_itree TicketLock.omod (SCMem.mod TicketLock.gvs)
+         (if x then Ret () else tau;; TicketLock.lock_loop (SCMem.val_nat mytk));;;
+       OMod.close_itree TicketLock.omod (SCMem.mod TicketLock.gvs) (trigger Yield))).
+  Proof.
+    iIntros "[#[CIH MONOTK] [MYN [MYTK [TKS [MEM [ST [I K]]]]]]]".
+    iPoseProof (mytk_find_some with "[MYTK TKS]") as "%FIND". iFrame.
+    iPoseProof (unlocked1_mono with "I") as "[%TKQ #[% [% [MONOW OBLB]]]]".
+    clear FIND TKQ.
+    iStopProof. move o before IH. revert_until o. pattern o. revert o.
+    apply (well_founded_induction Ord.lt_well_founded).
+    intros o IHo. intros.
+    iIntros "[#[CIH [MONOTK [MONOW BLK]]] [MYN [MYTK [TKS [MEM [ST [I K]]]]]]]".
+
+    unfold Mod.wrap_fun, SCMem.compare_fun. rred.
+    iDestruct "MEM" as "[MEM0 [MEM1 [MEM2 MEM3]]]". iDestruct "ST" as "[ST0 ST1]".
+    iApply stsim_getR. iSplit. eauto. rred.
+    iApply stsim_tauR. rred. iApply stsim_tauR. rred.
+    destruct (Nat.eq_dec now_old mytk).
+    { exfalso. clarify. }
+    rred. iApply stsim_tauR.
+    rewrite TicketLock.lock_loop_red. rred. rewrite close_itree_call. rred.
+    iAssert (ticket_lock_inv_mem mem now next myt)%I with "[MEM0 MEM1 MEM2 MEM3]" as "MEM". iFrame.
+    iAssert (ticket_lock_inv_state mem false tks)%I with "[ST0 ST1]" as "ST". iFrame.
+    iMod ("K" with "[TKS MEM ST I]") as "_".
+    { do 7 iExists _. iSplitL "TKS". iFrame. iSplitL "MEM". iFrame. iSplitL "ST". iFrame.
+      iRight. iSplit. auto. iRight. iRight. iFrame.
+    }
+    clear mem l tks next myt now_old NEQ n.
+    rename now into now_past, LT into LTPAST, k into k_past, o into o_past.
+
+    iopen 0 "I" "K". do 7 iDestruct "I" as "[% I]". iDestruct "I" as "[TKS [MEM [ST CASES]]]".
+    destruct (Nat.eq_dec mytk now); subst.
+    { iClear "CIH".
+      iApply lock_myturn1.
+      iSplitL "MYTK". iFrame. iSplitL "MYN". iFrame. iSplitL "TKS". iFrame.
+      iSplitL "MEM". iFrame. iSplitL "ST". iFrame. iSplitL "CASES". iFrame.
+      iFrame.
+    }
+
+    rename n into NEQ.
+    iApply lock_yourturn_yieldR. eapply NEQ.
+    iSplitL "MYTK TKS MEM ST CASES K".
+    iSplitL "MYTK". iFrame. iSplitL "TKS". iFrame. iSplitL "MEM". iFrame.
+    iSplitL "ST". iFrame. iSplitL "CASES". iFrame. iFrame.
+    iIntros "[MYTK _]". rred.
+    clear mem own l tks now next myt NEQ.
+    iopen 0 "I" "K". do 7 iDestruct "I" as "[% I]". iDestruct "I" as "[TKS [MEM [ST CASES]]]".
+    destruct (Nat.eq_dec mytk now); subst.
+    { iClear "CIH".
+      iPoseProof (mytk_find_some with "[MYTK TKS]") as "%FIND". iFrame.
+      iDestruct "CASES" as "[[%CT I] | [%CF [I | [I | I]]]]".
+      { iPoseProof (locked_contra with "I") as "%F". eauto. inv F. }
+      { iPoseProof (unlocking_contra with "I") as "%F". eauto. inv F. }
+      { iPoseProof (unlocked0_contra with "I") as "%F". eauto. inv F. }
+      iPoseProof (unlocked1_mono with "I") as "[%TKQ #[% [% [MYTN _]]]]".
+      iMod ("K" with "[TKS MEM ST I]") as "_".
+      { do 7 iExists _. iSplitL "TKS". iFrame. iSplitL "MEM". iFrame. iSplitL "ST". iFrame.
+        iRight. iSplit. auto. iFrame.
+      }
+      iApply lock_myturn0. 2: iFrame; auto. lia.
+    }
+
+    rename n into NEQ. unfold Mod.wrap_fun, SCMem.load_fun. rred.
+    iDestruct "MEM" as "[MEM0 [MEM1 [MEM2 MEM3]]]". iDestruct "ST" as "[ST0 ST1]".
+    iApply stsim_getR. iSplit. eauto. rred.
+    iApply stsim_tauR. rred.
+    iPoseProof (memory_ra_load with "MEM0 MEM1") as "%LOAD". des. rewrite LOAD. rred.
+    iApply stsim_tauR. rred.
+    rewrite close_itree_call. rred.
+    iApply lock_yourturn_yieldR. eapply NEQ.
+    iSplitL "MYTK TKS MEM0 MEM1 MEM2 MEM3 ST0 ST1 CASES K".
+    iSplitL "MYTK". iFrame. iSplitL "TKS". iFrame. iSplitL "MEM0 MEM1 MEM2 MEM3". iFrame.
+    iSplitL "ST0 ST1". iFrame. iSplitL "CASES". iFrame. iFrame.
+    iIntros "[MYTK RIGHT]". rred.
+    rename now into now_old. clear mem own l tks next myt LOAD LOAD0.
+
+    iopen 0 "I" "K". do 7 iDestruct "I" as "[% I]". iDestruct "I" as "[TKS [MEM [ST CASES]]]".
+    destruct (Nat.eq_dec mytk now); subst.
+    { iClear "CIH". iApply lock_myturn2. auto.
+      iSplitL "MYTK". iFrame. iSplitL "MYN". iFrame. iSplitL "TKS". iFrame.
+      iSplitL "MEM". iFrame. iSplitL "ST". iFrame. iSplitL "CASES". iFrame.
+      iFrame.
+    }
+
+    iPoseProof (mytk_find_some with "[MYTK TKS]") as "%FIND". iFrame.
+    rename n into NEQ2. iPoseProof (yourturn_range with "CASES") as "%LT". eapply FIND. auto.
+    clear NEQ2. iDestruct "CASES" as "[[%CT I] | [%CF [I | [I | I]]]]".
+    { subst own. iApply lock_yourturn_coind. auto. iSplit. iApply "CIH".
+      iSplitL "MYN". iFrame. iSplitL "MYTK". iFrame. iSplitL "TKS". iFrame.
+      iSplitL "MEM". iFrame. iSplitL "ST". iFrame. iSplitL "I". iFrame. iFrame.
+    }
+
+    { iPoseProof (ticket_lock_inv_mem_mono with "MEM") as "#MONOTK2".
+      iAssert (⌜now_past <= now⌝)%I with "[MEM]" as "%PROG".
+      { iDestruct "MEM" as "[MEM0 [MEM1 [MEM2 [MEM3 MEM4]]]]".
+        iPoseProof (black_white_compare with "MONOTK MEM4") as "%". auto.
+      }
+      iApply lock_yourturn_ind0. apply LT.
+      { clear IHo. move LT before IH. move PROG before LT. clear_upto PROG.
+        intros y H. eapply IH. lia.
+      }
+      auto.
+      iSplit.
+      { iClear "MYN MYTK RIGHT TKS MEM ST I K". iModIntro. iSplit. iApply "CIH". auto. }
+      iSplitL "MYN". iFrame. iSplitL "MYTK". iFrame. iSplitL "TKS". iFrame. iSplitL "MEM". iFrame.
+      iSplitL "ST". subst. iFrame. iSplitR "K". 2: iFrame.
+      iFrame.
+    }
+
+    { iPoseProof (unlocked0_contra with "I") as "%FF". eauto. inv FF. }
+
+    { iPoseProof (ticket_lock_inv_mem_mono with "MEM") as "#MONOTK2".
+      do 2 iDestruct "I" as "[% I]". iDestruct "I" as "[I0 [%I1 [%I2 [I3 [I4 I5]]]]]".
+      do 3 iDestruct "I5" as "[% I5]". iDestruct "I5" as "[I5 [I6 [I7 [I8 [I9 I10]]]]]".
+      iPoseProof (black_white_compare with "MONOW I5") as "%LE".
+      inv LE.
+      { remember (mytk - now) as ind. specialize (IH ind).
+        iApply IH.
+        { subst ind. lia. }
+        { auto. }
+        { eapply LT. }
+        { eapply Heqind. }
+        iSplit.
+        { iClear "MYN MYTK RIGHT TKS MEM ST I0 I3 I4 I5 I6 I7 I8 I9 I10 K".
+          iModIntro. iSplit. iApply "CIH". auto.
+        }
+        iSplitL "MYN". iFrame. iSplitL "MYTK". iFrame. iSplitL "TKS". iFrame.
+        iSplitL "ST". iFrame. iSplitR "K MEM". 2: iFrame.
+        iRight. iSplit. auto. iRight. iRight. iFrame. iExists yourt, waits.
+        iSplit. auto. iSplit. auto. iFrame. iExists k, o, u. iFrame.
+      }
+      { inv ORD. hexploit H0. lia. i. clear H H0. subst k.
+        iClear "MONOTK2".
+        iPoseProof (ObligationRA.duty_correl_thread with "I8") as "#COR".
+        { ss. left; eauto. }
+        iPoseProof (ObligationRA.correl_thread_correlate with "COR RIGHT") as ">[DROP | FF]".
+        2:{ iPoseProof (ObligationRA.pending_not_shot with "I7 FF") as "%FF". inv FF. }
+        iPoseProof (ObligationRA.black_white_decr with "BLK DROP") as ">[%o_now [#OBLK2 %DROP]]".
+        iClear "BLK".
+        specialize (IHo o_now). iApply IHo.
+        { rewrite Hessenberg.add_S_r in DROP. rewrite Hessenberg.add_O_r in DROP.
+          eapply Ord.lt_le_lt. 2: eapply DROP. apply Ord.S_lt.
+        }
+        { auto. }
+        iSplit.
+        { iClear "MYN MYTK TKS MEM ST I0 I3 I4 I5 I6 I7 I8 I9 I10 K".
+          iModIntro. iSplit. iApply "CIH". auto.
+        }
+        iSplitL "MYN". iFrame. iSplitL "MYTK". iFrame. iSplitL "TKS". iFrame.
+        iSplitL "MEM". iFrame. iSplitL "ST". iFrame. iSplitR "K". 2: iFrame.
+        iFrame. iExists yourt, waits.
+        iSplit. auto. iSplit. auto. iFrame. iExists _, _, u. iFrame.
+      }
+    }
+  Qed.
+
+  Lemma correct_lock tid:
+    ((own_thread tid)
+       ∗ (ObligationRA.duty (inl tid) [])
+    )
+      ⊢
+      (stsim I tid (topset I) ibot7 ibot7
+             (fun r_src r_tgt => own_thread tid ** ObligationRA.duty (inl tid) [] ** ⌜r_src = r_tgt⌝)
+             false false
+             (AbsLock.lock_fun tt)
+             (OMod.close_itree TicketLock.omod (SCMem.mod TicketLock.gvs)
+                               (TicketLock.lock_fun tt))).
+  Proof.
+    iIntros "[MYTH DUTY]".
+    iApply lock_enqueue. iSplitL. iFrame.
+    iIntros "% [MYTK MYN]".
+    rewrite TicketLock.lock_loop_red. rred. rewrite close_itree_call. rred.
+    iStopProof. revert mytk. eapply stsim_coind. msubtac.
+    iIntros "% %mytk". iIntros "#[_ CIH] [MYTK MYN]".
+
+    iopen 0 "I" "K". do 7 iDestruct "I" as "[% I]". iDestruct "I" as "[TKS [MEM [ST CASES]]]".
+    destruct (Nat.eq_dec mytk now); subst.
+    { iClear "CIH".
+      rewrite unfold_iter_eq. lred. iApply lock_myturn1.
+      iSplitL "MYTK". iFrame. iSplitL "MYN". iFrame. iSplitL "TKS". iFrame.
+      iSplitL "MEM". iFrame. iSplitL "ST". iFrame. iSplitL "CASES". iFrame.
+      iFrame.
+    }
+
+    rename n into NEQ. rewrite unfold_iter_eq. lred.
+    iApply lock_yourturn_yieldR. eapply NEQ.
+    iSplitL "MYTK TKS MEM ST CASES K".
+    iSplitL "MYTK". iFrame. iSplitL "TKS". iFrame. iSplitL "MEM". iFrame.
+    iSplitL "ST". iFrame. iSplitL "CASES". iFrame. iFrame.
+    iIntros "[MYTK _]". rred.
+    clear mem own l tks now next myt NEQ.
+    iopen 0 "I" "K". do 7 iDestruct "I" as "[% I]". iDestruct "I" as "[TKS [MEM [ST CASES]]]".
+    destruct (Nat.eq_dec mytk now); subst.
+    { iClear "CIH".
+      iPoseProof (mytk_find_some with "[MYTK TKS]") as "%FIND". iFrame.
+      iDestruct "CASES" as "[[%CT I] | [%CF [I | [I | I]]]]".
+      { iPoseProof (locked_contra with "I") as "%F". eauto. inv F. }
+      { iPoseProof (unlocking_contra with "I") as "%F". eauto. inv F. }
+      { iPoseProof (unlocked0_contra with "I") as "%F". eauto. inv F. }
+      iPoseProof (unlocked1_mono with "I") as "[%TKQ #[% [% [MYTN _]]]]".
+      iMod ("K" with "[TKS MEM ST I]") as "_".
+      { do 7 iExists _. iSplitL "TKS". iFrame. iSplitL "MEM". iFrame. iSplitL "ST". iFrame.
+        iRight. iSplit. auto. iFrame.
+      }
+      iApply lock_myturn0. 2: iFrame; auto. lia.
+    }
+
+    rename n into NEQ.
+    unfold Mod.wrap_fun, SCMem.load_fun. rred.
+    iDestruct "MEM" as "[MEM0 [MEM1 [MEM2 MEM3]]]". iDestruct "ST" as "[ST0 ST1]".
+    iApply stsim_getR. iSplit. eauto. rred.
+    iApply stsim_tauR. rred.
+    iPoseProof (memory_ra_load with "MEM0 MEM1") as "%LOAD". des. rewrite LOAD. rred.
+    iApply stsim_tauR. rred.
+    rewrite close_itree_call. rred.
+    iApply lock_yourturn_yieldR. eapply NEQ.
+    iSplitL "MYTK TKS MEM0 MEM1 MEM2 MEM3 ST0 ST1 CASES K".
+    iSplitL "MYTK". iFrame. iSplitL "TKS". iFrame. iSplitL "MEM0 MEM1 MEM2 MEM3". iFrame.
+    iSplitL "ST0 ST1". iFrame. iSplitL "CASES". iFrame. iFrame.
+    iIntros "[MYTK _]". rred.
+    rename now into now_old. clear mem own l tks next myt LOAD LOAD0.
+
+    iopen 0 "I" "K". do 7 iDestruct "I" as "[% I]". iDestruct "I" as "[TKS [MEM [ST CASES]]]".
+    destruct (Nat.eq_dec mytk now); subst.
+    { iClear "CIH". iApply lock_myturn2. auto.
+      iSplitL "MYTK". iFrame. iSplitL "MYN". iFrame. iSplitL "TKS". iFrame.
+      iSplitL "MEM". iFrame. iSplitL "ST". iFrame. iSplitL "CASES". iFrame.
+      iFrame.
+    }
+
+    rename n into NEQ2.
+    iPoseProof (mytk_find_some with "[MYTK TKS]") as "%FIND". iFrame.
+    iDestruct "MEM" as "[MEM0 [MEM1 [MEM2 [MEM3 MEM4]]]]".
+    iPoseProof (black_white with "MEM4") as "#MONOTK".
+    iAssert (ticket_lock_inv_mem mem now next myt)%I with "[MEM0 MEM1 MEM2 MEM3 MEM4]" as "MEM".
+    iFrame.
+    iPoseProof (yourturn_range with "CASES") as "%LT". eapply FIND. auto.
+    clear FIND NEQ2.
+    remember (mytk - now) as ind.
+    iStopProof. move ind before mytk. revert_until ind. pattern ind. revert ind.
+    apply (well_founded_induction Nat.lt_wf_0).
+    intros ind IH. intros.
+    iIntros "[#[CIH MONOTK] [MYN [MYTK [TKS [ST [CASES [K MEM]]]]]]]".
+
+    iDestruct "CASES" as "[[%CT I] | [%CF [I | [I | I]]]]".
+    { subst own. iApply lock_yourturn_coind. auto. iSplit. iApply "CIH".
+      iSplitL "MYN". iFrame. iSplitL "MYTK". iFrame. iSplitL "TKS". iFrame.
+      iSplitL "MEM". iFrame. iSplitL "ST". iFrame. iSplitL "I". iFrame. iFrame.
+    }
+    { subst. iApply lock_yourturn_ind0. apply LT. apply IH. auto.
+      iSplit.
+      { iClear "MYN MYTK TKS MEM ST I K".
+        iModIntro. iSplit. iApply "CIH". auto.
+      }
+      iSplitL "MYN". iFrame. iSplitL "MYTK". iFrame. iSplitL "TKS". iFrame.
+      iSplitL "MEM". iFrame. iSplitL "ST". iFrame. iSplitR "K". 2: iFrame.
+      iFrame.
+    }
+    { iPoseProof (mytk_find_some with "[MYTK TKS]") as "%FIND". iFrame.
+      iPoseProof (unlocked0_contra with "I") as "%FF". eauto. inv FF.
+    }
+    { subst. iApply lock_yourturn_ind1. apply LT. apply IH. auto.
+      iSplit.
+      { iClear "MYN MYTK TKS MEM ST I K". iModIntro. iSplit. iApply "CIH". auto. }
+      iSplitL "MYN". iFrame. iSplitL "MYTK". iFrame. iSplitL "TKS". iFrame.
+      iSplitL "MEM". iFrame. iSplitL "ST". iFrame. iSplitR "K". 2: iFrame.
+      iFrame.
+    }
+
+  Qed.
+
+  Lemma correct_unlock tid:
+    ((own_thread tid)
+       ∗ (ObligationRA.duty (inl tid) [])
+    )
+      ⊢
+      (stsim I tid (topset I) ibot7 ibot7
+             (fun r_src r_tgt => own_thread tid ** ObligationRA.duty (inl tid) [] ** ⌜r_src = r_tgt⌝)
+             false false
+             (AbsLock.unlock_fun tt)
+             (OMod.close_itree TicketLock.omod (SCMem.mod TicketLock.gvs)
+                               (TicketLock.unlock_fun tt))).
+  Proof.
+    iIntros "[MYTH DUTY]".
+    unfold AbsLock.unlock_fun, TicketLock.unlock_fun. rred.
+    rewrite close_itree_call. rred.
+    iApply (stsim_sync with "[DUTY]"). msubtac. iFrame. iIntros "DUTY _".
+    iopen 0 "I" "K". do 7 iDestruct "I" as "[% I]". iDestruct "I" as "[TKS [MEM [ST CASES]]]".
+    iDestruct "CASES" as "[[%CT I] | [%CF [I | [I | I]]]]"; cycle 1.
+    { subst own. iDestruct "ST" as "[ST0 ST1]".
+      iApply stsim_getL. iSplit. auto. rred.
+      destruct (Bool.eqb false true) eqn:BEQ. exfalso. inv BEQ.
+      iApply stsim_UB.
+    }
+    { subst own. iDestruct "ST" as "[ST0 ST1]".
+      iApply stsim_getL. iSplit. auto. rred.
+      destruct (Bool.eqb false true) eqn:BEQ. exfalso. inv BEQ.
+      iApply stsim_UB.
+    }
+    { subst own. iDestruct "ST" as "[ST0 ST1]".
+      iApply stsim_getL. iSplit. auto. rred.
+      destruct (Bool.eqb false true) eqn:BEQ. exfalso. inv BEQ.
+      iApply stsim_UB.
+    }
+
+    subst own. iDestruct "ST" as "[ST0 ST1]".
+    iApply stsim_getL. iSplit. auto. rred.
+    destruct (Bool.eqb true true) eqn:BEQ. 2: exfalso; inv BEQ.
+    clear BEQ.
+    iApply (stsim_putL with "ST1"). iIntros "ST1".
+
+    unfold Mod.wrap_fun, SCMem.load_fun. rred.
+    iDestruct "MEM" as "[MEM0 [MEM1 [MEM2 [MEM3 MEM4]]]]".
+    iApply stsim_getR. iSplit. eauto. rred.
+    iApply stsim_tauR. rred.
+    iPoseProof (memory_ra_load with "MEM0 MEM1") as "%LOAD". des. rewrite LOAD. rred.
+    iApply stsim_tauR. rred.
+    rewrite close_itree_call. rred.
+
+    iPoseProof (ObligationRA.alloc (((Ord.S Ord.O) × Ord.omega) × (Ord.from_nat 2))%ord) as "> [% [[OBLK OWHI] OPEND]]".
+    iPoseProof (ObligationRA.white_eq with "OWHI") as "OWHI".
+    { rewrite Ord.from_nat_S. rewrite Jacobsthal.mult_S. reflexivity. }
+    iPoseProof (ObligationRA.white_split_eq with "OWHI") as "[OWHI TAX]".
+    iPoseProof (ObligationRA.duty_alloc with "DUTY OWHI") as "> DUTY".
+
+    iDestruct "I" as "[I0 [I1 [I2 [I3 [% I5]]]]]".
+    iPoseProof (black_updatable with "I5") as ">I5".
+    { instantiate (1:=(now, Tkst.d k)). econs 2. ss. split; try lia. }
+    iPoseProof (black_white_update with "MEM3 I0") as ">[MEM3 HOLD]". instantiate (1:=(now, tid)).
+
+    iApply (stsim_yieldR_strong with "[DUTY TAX]").
+    { iSplitL "DUTY". iFrame. iApply ObligationRA.tax_cons_fold. iSplit. 2: auto.
+      iApply ObligationRA.white_eq. 2: iFrame.
+      rewrite Ord.from_nat_1. rewrite Jacobsthal.mult_1_r. reflexivity.
+    }
+    iIntros "DUTY _".
+    iMod ("K" with "[MYTH TKS MEM0 MEM1 MEM2 MEM3 MEM4 ST0 ST1 I1 I2 I3 I5 OBLK OPEND DUTY]") as "_".
+    { iExists mem, false, l, tks, now, next, tid.
+      remember (
+    (⌜false = true⌝ ** ticket_lock_inv_locked l tks now next tid)
+    ∨ (⌜false = false⌝ **
+       ticket_lock_inv_unlocking l tks now next tid
+       ∨ ticket_lock_inv_unlocked0 l tks now next tid
+       ∨ ticket_lock_inv_unlocked1 l tks now next tid))%I as temp.
+      iFrame. subst temp.
+      iRight. iSplit. auto. iLeft. iFrame.
+      iExists _, _. iFrame.
+    }
+    iModIntro. clear_upto tid.
+
+    iopen 0 "I" "K". do 7 iDestruct "I" as "[% I]". iDestruct "I" as "[TKS [MEM [ST CASES]]]".
+    iDestruct "CASES" as "[[%CT I] | [%CF [I | [I | I]]]]"; cycle 2.
+    { iDestruct "I" as "[I _]". iPoseProof (white_white_excl with "HOLD I") as "%FF". inv FF. }
+    { do 2 iDestruct "I" as "[% I]". iDestruct "I" as "[I _]".
+      iPoseProof (white_white_excl with "HOLD I") as "%FF". inv FF. }
+    { iDestruct "I" as "[I _]". iPoseProof (white_white_excl with "HOLD I") as "%FF". inv FF. }
+
+    unfold Mod.wrap_fun, SCMem.store_fun. rred.
+    iDestruct "ST" as "[ST0 ST1]". iDestruct "MEM" as "[MEM0 [MEM1 [MEM2 [MEM3 MEM4]]]]".
+    iApply stsim_getR. iSplit. auto. rred.
+    iApply stsim_tauR. rred.
+    iPoseProof (memory_ra_store with "MEM0 MEM1") as "[% [%STORE >[MEM0 MEM1]]]".
+    rewrite STORE. rred.
+    iApply stsim_getR. iSplit. auto. rred.
+    iApply (stsim_putR with "ST0"). iIntros "ST0". rred.
+    iApply stsim_tauR. rred. iApply stsim_tauR. rred.
+
+    iPoseProof (black_white_equal with "MEM3 HOLD") as "%EQ". inv EQ.
+    remember (S now) as now'.
+    replace (now + 1) with now'. 2: lia.
+    iPoseProof (black_white_update with "MEM3 HOLD") as ">[MEM3 HOLD]". instantiate (1:=(now', tid)).
+    iPoseProof (black_updatable with "MEM4") as ">MEM4".
+    { instantiate (1:=now'). lia. }
+    iDestruct "I" as "[I1 [%I2 [I3 [I4 I5]]]]".
+    do 2 iDestruct "I5" as "[% I5]". iDestruct "I5" as "[I5 [_ [OPEND DUTY]]]".
+    iPoseProof (ObligationRA.pending_shot with "OPEND") as ">OSHOT".
+    iPoseProof (ObligationRA.duty_done with "DUTY OSHOT") as ">DUTY".
+
+    destruct l as [ | yourt waits].
+    { iPoseProof (black_updatable with "I5") as ">I5".
+      { instantiate (1:=(now', Tkst.a k)). econs 1; try lia. }
+      iAssert (ticket_lock_inv_mem m1 now' next tid)%I with "[MEM0 MEM1 MEM2 MEM3 MEM4]" as "MEM".
+      iFrame.
+      iAssert (ticket_lock_inv_state m1 false tks)%I with "[ST0 ST1]" as "ST". iFrame.
+      iMod ("K" with "[TKS MEM ST I3 I4 I5 HOLD]") as "_".
+      { do 7 iExists _. iSplitL "TKS". iFrame. iSplitL "MEM". iFrame. iSplitL "ST". iFrame.
+        iRight. iSplit. auto. iRight. iLeft. iFrame. iSplit.
+        iPureIntro. split; eauto. inv I2; ss.
+        iExists _. iFrame.
+      }
+      iApply (stsim_sync with "[DUTY]"). msubtac. iFrame. iIntros "DUTY _".
+      iApply stsim_tauR.
+      iApply stsim_ret. iModIntro. iFrame. auto.
+    }
+
+    iPoseProof (list_prop_sum_cons_unfold with "I4") as "[[YDUTY [% YMAPS]] I4]".
+    iPoseProof (ObligationRA.alloc (((Ord.S Ord.O) × Ord.omega) × (Ord.S (Ord.from_nat u)))%ord) as "> [% [[OBLK OWHI] OPEND]]".
+    iPoseProof (ObligationRA.white_eq with "OWHI") as "OWHI".
+    { rewrite Jacobsthal.mult_S. reflexivity. }
+    iPoseProof (ObligationRA.white_split_eq with "OWHI") as "[OWHI YTAX]".
+    iPoseProof (ObligationRA.duty_alloc with "YDUTY OWHI") as "> YDUTY".
+
+    iPoseProof (black_updatable with "I5") as ">I5".
+    { instantiate (1:=(now', Tkst.b k0)). econs 1; try lia. }
+    iAssert (ticket_lock_inv_mem m1 now' next tid)%I with "[MEM0 MEM1 MEM2 MEM3 MEM4]" as "MEM".
+    iFrame.
+    iAssert (ticket_lock_inv_state m1 false tks)%I with "[ST0 ST1]" as "ST". iFrame.
+    iMod ("K" with "[TKS MEM ST I3 HOLD YMAPS I4 OBLK OPEND YTAX YDUTY I5]") as "_".
+    { subst now'. do 7 iExists _. iSplitL "TKS". iFrame. iSplitL "MEM". iFrame.
+      iSplitL "ST". iFrame. iRight. iSplit. auto. iRight. iRight. iExists yourt, waits.
+      iFrame. iSplit. auto. iSplit. auto.
+      iExists k0, _, u. iFrame.
+    }
+    iApply (stsim_sync with "[DUTY]"). msubtac. iFrame. iIntros "DUTY _".
+    iApply stsim_tauR.
+    iApply stsim_ret. iModIntro. iFrame. auto.
+
+  Qed.
 
 
 
